theories/deque_corr.v
@@ -1,0 +1,477 @@
+From iris.heap_lang Require Import lang proofmode notation.
+From iris.bi Require Import derived_laws.
+
+From Coq Require Import List.
+Import ListNotations.
+
+From AAC_tactics Require Import AAC.
+From AAC_tactics Require Import Instances.
+Import Instances.Lists.
+
+From Deque Require Import common tick shared_ref.
+
+Section concurrent_deques.
+  (* This section describes the structure used for the proof of the concurrent correction *)
+
+  Context `{!heapGS Σ}.
+
+  Let isDequeType := list val -d> val -d> iProp Σ.
+
+  Let fFiveTuple (triple_pred : isDequeType) (deque_pred : isDequeType) : isDequeType := (
+    λ o d, ∃ (pr ld md rd sf : val)
+      pr_content left_content md_content right_content sf_content
+      (kPr kMd kSf : nat) left_triples right_triples,
+      ⌜ d = (pr, ld, md, rd, sf)%V ⌝ ∗
+      ⌜ five_tuple_configuration kPr (length left_content) kMd (length right_content) kSf ⌝ ∗
+      buffer kPr pr_content pr ∗
+      deque_pred left_triples ld ∗
+      buffer kMd md_content md ∗
+      deque_pred right_triples rd ∗
+      buffer kSf sf_content sf ∗
+      ([∗list] c;tr ∈ left_content;left_triples, ▷ triple_pred c tr) ∗
+      ([∗list] c;tr ∈ right_content;right_triples, ▷ triple_pred c tr) ∗
+      ⌜ o = pr_content ++ List.concat left_content ++ md_content ++ List.concat right_content ++ sf_content ⌝
+  )%I.
+
+  (* Define the mutual fixpoint functions *)
+  Let fDeque (triple_pred : isDequeType) (deque_pred : isDequeType) : isDequeType := (
+    λ o d,
+      (⌜ d = NONEV ∧ o = [] ⌝) ∨
+      (∃ ℓ : loc, ⌜ d = SOMEV #ℓ ⌝ ∗
+        ℓ ⤇ fFiveTuple triple_pred deque_pred o)
+  )%I.
+
+  Let fTriple (triple_pred : isDequeType) (deque_pred : isDequeType) : isDequeType := (
+    λ o t,
+      ∃ (fst ch lst : val)
+        fst_content child_content lst_content
+        (kFst kLst : nat) triples,
+        ⌜ triple_configuration kFst (length child_content) kLst ⌝ ∗
+        ⌜ t = (fst, ch, lst)%V ⌝ ∗
+        buffer kFst fst_content fst ∗
+        deque_pred triples ch ∗
+        buffer kLst lst_content lst ∗
+        ([∗list] c;tr ∈ child_content;triples, ▷ triple_pred c tr) ∗
+        ⌜ o = fst_content ++ List.concat child_content ++ lst_content ⌝
+  )%I.
+
+  (* Prove contractivity *)
+  Local Instance fDeque_contractive :
+    ∀ n, Proper (dist_later n ==> dist_later n ==> dist n) fDeque.
+  Proof.
+    intros k deque1 deque2 Hdist_cad triple1 triple2 Hdist_tri.
+    intros o d.
+    rewrite /fDeque.
+    do 4 (f_contractive || f_equiv).
+    rewrite /csref.
+    do 4 (f_contractive || f_equiv).
+    rewrite /fFiveTuple.
+    do 33 (f_contractive || f_equiv).
+    f_equiv. by apply (Hdist_tri _ _).
+    f_equiv.
+    f_equiv. by apply (Hdist_tri _ _).
+    f_equiv.
+    do 6 f_equiv. by apply (Hdist_cad _ _).
+    f_equiv. by apply (Hdist_cad _ _).
+  Qed.
+
+  Local Instance fTriple_contractive :
+    ∀ n, Proper (dist_later n ==> dist n ==> dist n) fTriple.
+  Proof.
+    intros k tr1 tr2 Hdist_tri de1 de2 Hdist_cad.
+    intros o t.
+    rewrite /fTriple.
+    do 21 (f_contractive || f_equiv).
+    - f_equiv. by apply (Hdist_cad _ _).
+      f_equiv.
+    do 5 f_equiv. f_contractive. by apply (Hdist_tri _ _).
+  Qed.
+
+  Definition triple := fixpoint_A fTriple fDeque.
+  Definition isDeque := fixpoint_B fTriple fDeque.
+  Definition fiveTuple := fFiveTuple triple isDeque.
+  Definition IsDeque o d := isDeque o d.
+
+  Definition isLaterFiveTuple : isDequeType := (
+    λ o d, ∃ (pr ld md rd sf : val)
+      pr_content left_content md_content right_content sf_content
+      (kPr kMd kSf : nat) left_triples right_triples,
+      ⌜ d = (pr, ld, md, rd, sf)%V ⌝ ∗
+      ⌜ five_tuple_configuration kPr (length left_content) kMd (length right_content) kSf ⌝ ∗
+      buffer kPr pr_content pr ∗
+      isDeque left_triples ld ∗
+      buffer kMd md_content md ∗
+      isDeque right_triples rd ∗
+      buffer kSf sf_content sf ∗
+      ([∗list] c;tr ∈ left_content;left_triples, triple c tr) ∗
+      ([∗list] c;tr ∈ right_content;right_triples, triple c tr) ∗
+      ⌜ o = pr_content ++ List.concat left_content ++ md_content ++ List.concat right_content ++ sf_content ⌝
+  )%I.
+
+  (* Unfolding lemmas come directly from the fixpoint theory *)
+  Lemma isDeque_unfold o d :
+    isDeque o d ⊣⊢ fDeque triple isDeque o d.
+  Proof.
+    symmetry.
+    apply (fixpoint_B_unfold fTriple fDeque _ _).
+  Qed.
+
+  Lemma triple_unfold o t :
+    triple o t ⊣⊢ fTriple triple isDeque o t.
+  Proof.
+    symmetry.
+    apply (fixpoint_A_unfold fTriple fDeque _ _).
+  Qed.
+
+  Global Instance isDequePersistent o d : Persistent (isDeque o d).
+  Proof.
+    rewrite isDeque_unfold /fDeque.
+    apply _.
+  Qed.
+
+  Global Instance triplePersistent o t : Persistent (triple o t).
+  Proof.
+    rewrite /triple /fixpoint_A /ofe.fixpoint_AB.
+    revert o t. apply fixpoint_ind.
+    - intros f1 f2 H P o t. rewrite -(H _ _) //.
+    - exists (λ _ _, emp)%I. apply _.
+    - intros.
+      rewrite /ofe.fixpoint_AA /fTriple /ofe.fixpoint_AB.
+      assert (forall a b, Persistent (fixpoint (fDeque x) a b)); [| apply _].
+      intros. apply fixpoint_ind.
+        + intros f1 f2 H' P'. rewrite -(H' _ _) //.
+        + exists (λ _ _, emp)%I. apply _.
+        + apply _.
+        + apply bi.limit_preserving_Persistent.
+          intros k f1 f2 Hdist. apply (Hdist _ _).
+    - apply limit_preserving_forall => o.
+      apply limit_preserving_forall => t.
+      apply bi.limit_preserving_Persistent.
+      intros k f1 f2 Hdist. apply (Hdist _ _).
+  Qed.
+
+  Global Instance fiveTuplePersistent o d : Persistent (fiveTuple o d).
+  Proof.
+    apply _.
+  Qed.
+
+  Lemma laterInFiveTuple : forall o d, isLaterFiveTuple o d ⊢ fiveTuple o d.
+  Proof.
+    iIntros (o d) "(%pr & %ld & %md & %rd & %sf & %prC & %ldC & %mdC & %rdC & %sfC
+            & %kPr & %kMd & %kSf & %ltr & %rtr & -> & %cfg
+            & #Hpr & #Hld & #Hmd & #Hrd & #Hsf & #Hltr & #Hrtr & #Heq)".
+    iExists pr, ld, md, rd, sf, prC, ldC, mdC, rdC, sfC, kPr, kMd, kSf, ltr, rtr; iFrame "#"; iFrame.
+    do 2 (iSplitR; [ done |]).
+    iSplitL "Hltr". iApply (big_sepL2_mono with "Hltr"). by auto.
+                    iApply (big_sepL2_mono with "Hrtr"). by auto.
+  Qed.
+
+End concurrent_deques.
+
+(* Useful tactics used throughout proofs (out of a section to be exported) *)
+Ltac ℓisDeque ℓ := rewrite !isDeque_unfold; iRight; iExists ℓ; iSplitR; [done |].
+Ltac isEmptyDeque := rewrite !isDeque_unfold; iLeft; iPureIntro; done.
+Ltac invert_all_in :=
+  repeat match goal with
+  | H : _ ∈ _ |- _ =>
+    first
+    [ inversion H; clear H; auto 10 with find_in_list
+    | inversion H; clear H; [ by contradiction |]
+    | by inversion H
+    ];
+    try contradiction
+  end.
+Ltac doneL := iSplitR; [done |].
+Ltac doneR := iSplitL; [| done].
+Ltac easy_config := try iPureIntro; constructor; list_elem_of.
+
+Section proofs.
+  (* This section contains lemmas used for the three main proofs, found in separate files. *)
+
+  Context `{!heapGS Σ}.
+
+  Lemma bool_decide_code_true (a : nat) (b : nat) : bool_decide (a = b) = true -> bool_decide (#a = #b) = true.
+  Proof.
+    intro.
+    apply bool_decide_eq_true_1 in H.
+    by apply bool_decide_eq_true_2, f_equal, f_equal, f_equal.
+  Qed.
+
+  Lemma bool_decide_code_false (a : nat) (b : nat) : bool_decide (a = b) = false -> bool_decide (#a = #b) = false.
+  Proof.
+    intro.
+    apply bool_decide_eq_false_1 in H.
+    apply bool_decide_eq_false_2.
+    intro. apply H.
+    inversion H0.
+    by apply Nat2Z.inj'.
+  Qed.
+
+  Example singleton_deque_spec : forall x : val,
+    {{{ emp }}} asingleton x {{{ d, RET d; IsDeque (⋅x) d }}}.
+  Proof.
+    iIntros (x Φ) "_ Hψ".
+    rewrite /asingleton. wp_pures.
+    wp_bind (bpush _ _)%E.
+    wp_apply (bpush_spec) as "%b #Hb".
+      { iApply bempty_spec. }
+    wp_pures.
+    wp_bind (ref _)%E.
+    wp_apply (csref_alloc (fiveTuple (⋅ x))) as "%ℓ Hℓ".
+      { rewrite /fiveTuple.
+        iExists bempty, empty, bempty, empty, b,
+                []          , []   , []          , []    , (⋅x),
+                0, 0, 1, [], [].
+        rewrite //=.
+        iSplitL. rewrite //.
+        iSplitL. iPureIntro. constructor. list_elem_of.
+        iSplitL. iApply bempty_spec.
+        iSplitL. isEmptyDeque.
+        iSplitL. iApply bempty_spec.
+        iSplitL. isEmptyDeque.
+        iFrame "#". done.
+      }
+    wp_pures.
+    iApply "Hψ".
+    iModIntro.
+    rewrite /IsDeque. ℓisDeque ℓ.
+    done.
+  Qed.
+
+  Lemma singleton_deque_better : forall x b, buffer 1 (⋅x) b -∗ fiveTuple (⋅ x) (bempty, NONEV, bempty, NONEV, b)%V.
+  Proof.
+    iIntros (x b) "#Hb".
+    iExists bempty, empty, bempty, empty, b,
+            []           , []    , []   , [], (⋅x),
+            0, 0, 1, [], [].
+    rewrite /=.
+    iSplitR. rewrite //.
+    iSplitR. iPureIntro. constructor. list_elem_of.
+    iSplitR. by iApply bempty_spec.
+    iSplitR. isEmptyDeque.
+    iSplitR. by iApply bempty_spec.
+    iSplitR. isEmptyDeque.
+    iSplitL; done.
+  Qed.
+
+  (* NOTE(Juliette): bring back?
+  Lemma bempty_is_empty : forall b o, buffer 0 o b ⊢ ⌜ o = [] ⌝.
+  Proof.
+    iIntros (b o) "H".
+    iDestruct "H" as "[_ %Heq]". iPureIntro; by apply nil_length_inv.
+  Qed.
+  *)
+
+  (*
+  Lemma push_buffer_element_spec x b : forall n o oX size,
+    {{{ isElement π n oX x ∗ buffer π size n o b }}}
+      bpush x b
+    {{{ b', RET b'; buffer π (S size) n (oX ++ o) b' }}}.
+  Proof.
+    destruct n; iIntros (o oX size ψ) "[Hx Hb] Hψ".
+    - iCombine "Hx Hb" as "[-> [Hb %sEqL]]".
+      wp_apply (bpush_spec with "Hb") as "%b' Hb'".
+      iApply "Hψ".
+      iSplitL. done.
+      iPureIntro. simpl; auto.
+    - rewrite /isElement.
+      iDestruct "Hb" as "(%triples & %triples_content & Hb & [%Ho %lenEqSz] & areTriples)".
+      wp_apply (bpush_spec with "Hb") as "%b' Hb'".
+      iApply "Hψ".
+      rewrite /buffer /buffer.
+      iExists (⋅ x ++ triples), (⋅ oX ++ triples_content).
+      iFrame. iSplitR.
+      + iPureIntro; split.
+        * rewrite /= Ho //.
+        * rewrite /= lenEqSz //.
+      + iSplitR. done.
+        iApply (big_sepL2_mono with "areTriples").
+        intros. iIntros "t". by iNext.
+  Qed.
+
+  Corollary inject_buffer_element_spec x b : forall n o oX size,
+    {{{ isElement π n oX x ∗ buffer π size n o b }}}
+      binject b x
+    {{{ b', RET b'; buffer π (S size) n (o ++ oX) b' }}}.
+  Admitted.
+
+  Lemma pop_buffer_element_spec b : forall n o size,
+    {{{ buffer π (S size) n o b }}}
+      bpop b
+    {{{ x b', RET (x, b'); ∃ oX o', buffer π size n o' b' ∗ ⌜ o = oX ++ o' ⌝ ∗ isElement π n oX x }}}.
+  Proof.
+    destruct n; iIntros (o size ψ) "Hb Hψ".
+    - iDestruct "Hb" as "[Hb %sEqL]".
+      destruct o. by inversion sEqL.
+      wp_apply (bpop_spec with "Hb") as "%b' Hb'".
+      iApply "Hψ".
+      iExists (⋅ v).
+      iFrame. iSplit; iPureIntro.
+      + by inversion sEqL.
+      + auto.
+    - iDestruct "Hb" as "(%triples & %triples_content & Hb & [%Ho %lenEqSz] & areTriples)".
+      destruct triples. by inversion lenEqSz.
+      iDestruct (big_sepL2_length with "areTriples") as "%Hlen".
+      destruct triples_content. by rewrite lenEqSz // in Hlen.
+      wp_apply (bpop_spec with "Hb") as "%b' Hb'".
+      iApply "Hψ".
+      iDestruct (big_sepL2_cons with "areTriples") as "[tri Hrest]".
+      iExists l, (List.concat triples_content).
+      iSplitL "Hb' Hrest".
+      + iExists triples, triples_content.
+        iSplitL "Hb'". done.
+        iSplitR.
+        * iPureIntro; split; [trivial |].
+          by inversion lenEqSz.
+        * iApply (big_sepL2_mono with "Hrest").
+          intros. iIntros "t". by iNext.
+      + iSplitR.
+        * iPureIntro. by rewrite Ho //.
+        * done.
+  Qed.
+
+   Corollary eject_buffer_element_spec b : forall n o size,
+    {{{ buffer π (S size) n o b }}}
+      beject b
+    {{{ b' x, RET (b', x); ∃ oX o', buffer π size n o' b' ∗ ⌜ o = o' ++ oX ⌝ ∗ isElement π n oX x }}}.
+  Admitted.
+
+  Ltac solve_no_middle Heq H H1 :=
+  iSplitR; [done |];
+  iSplitR; [iPureIntro; constructor; list_elem_of |];
+  iSplitL "ι"; [iExact "ι" |];
+  iSplitR; [trivial |];
+  iSplitR; [isEmptyDeque |];
+  iSplitR; [trivial |];
+  iSplitR; [isEmptyDeque |];
+  iSplitR; [trivial |];
+  inversion cfg;
+  [ rewrite Heq;
+    symmetry in H, H1;
+    iDestruct (bempty_is_empty with "Hpr") as "->";
+    iDestruct (bempty_is_empty with "Hmd") as "->";
+    rewrite (nil_length_inv _ H);
+    rewrite (nil_length_inv _ H1);
+    iPureIntro;
+    aac_reflexivity
+  | inversion H0; inversion H8; inversion H12; inversion H16; inversion H20
+  ].
+  *)
+
+  (*
+  Lemma bpush_spec2 x b : forall o size,
+    {{{ buffer size o b }}}
+      bpush x b
+    {{{ b', RET b'; buffer (S size) (⋅x ++ o) b' }}}.
+  Proof.
+    iIntros (o size ψ) "[Hb %Heq] Hψ".
+    wp_apply (bpush_spec with "Hb") as "%b' Hb'".
+    iApply "Hψ".
+    iFrame. iPureIntro. simpl. by rewrite Heq //.
+  Qed.
+
+  Corollary binject_spec2 b x : forall o size,
+    {{{ buffer size o b }}}
+      binject b x
+    {{{ b', RET b'; buffer (S size) (o ++ ⋅x) b' }}}.
+  Admitted.
+
+  Lemma bpop_spec2 b : forall o size,
+    {{{ buffer (S size) o b }}}
+      bpop b
+    {{{ x b' o', RET (x, b'); buffer size o' b' ∗ ⌜ o = ⋅x ++ o' ⌝ }}}.
+  Proof.
+    iIntros (o size ψ) "[Hb %Heq] Hψ".
+    destruct o. by inversion Heq.
+    wp_apply (bpop_spec with "Hb") as "%b' Hb'".
+    iApply "Hψ". iFrame.
+    iPureIntro. by inversion Heq.
+  Qed.
+
+  Corollary beject_spec2 b : forall o size,
+    {{{ buffer (S size) o b }}}
+      beject b
+    {{{ b' x o', RET (b', x); buffer size o' b' ∗ ⌜ o = o' ++ ⋅x ⌝ }}}.
+  Admitted.
+  *)
+
+  Lemma decrease_in : forall n o, n ∈ map S o -> ∃ k, n = k + 1 ∧ k ∈ o.
+  Proof.
+    induction o; intros.
+    - inversion H.
+    - rewrite /= in H.
+      inversion H.
+      + exists a. split; [ auto | list_elem_of ]. lia.
+      + specialize (IHo H2) as (k & G1 & G2).
+        exists k. split; [ auto | list_elem_of ].
+  Qed.
+
+  (*
+  Property partition_buffer_left_better_spec : forall k o b,
+    {{{ buffer k o b ∗ ⌜ k ∈ [2..6] ⌝ }}}
+      partition_buffer_left b
+    {{{ b1 b2 o1 o2 k1 k2, RET (b1, b2)%V;
+        buffer k1 o1 b1 ∗ buffer k2 o2 b2 ∗
+        ⌜ k1 ∈ [2; 3] ∧ k2 ∈ [0; 2; 3] ∧ o1 ++ o2 = o ⌝ }}}.
+  Proof.
+    iIntros (k o b ψ) "[[#Hb <-] %Hk] Hψ".
+      wp_apply partition_buffer_left_spec as (b1 b2) "(%o1 & %o2 & Hb1 & Hb2 & (%Hl1 & %Hl2 & <-))".
+        by iFrame "#".
+      iApply "Hψ".
+      by iFrame.
+  Qed.
+
+  Property partition_buffer_right_better_spec : forall k o b,
+    {{{ buffer k o b ∗ ⌜ k ∈ [2..6] ⌝ }}}
+      partition_buffer_right b
+    {{{ b1 b2 o1 o2 k1 k2, RET (b1, b2)%V;
+        buffer k1 o1 b1 ∗ buffer k2 o2 b2 ∗
+        ⌜ k1 ∈ [0; 2; 3] ∧ k2 ∈ [2; 3] ∧ o1 ++ o2 = o ⌝ }}}.
+  Admitted.
+  *)
+
+  Lemma lookup_triple (L : list (list val)) (M : list val) y :
+    y ∈ M -> ([∗ list] x;y ∈ L;M, triple x y)
+    ⊢ ∃ x, triple x y.
+  Proof.
+    revert M. induction L; iIntros (M H) "LM".
+    - iExFalso.
+      iDestruct (big_sepL2_nil_inv_l with "LM") as "->".
+      inversion H.
+    - destruct M. by inversion H.
+      iDestruct (big_sepL2_cons with "LM") as "[t LM]".
+      inversion H.
+      + by iExists a.
+      + by iApply (IHL M H2).
+  Qed.
+
+  Lemma abuffer_spec_explicit : forall n o b,
+    n ∈ [2; 3] -> {{{ buffer n o b }}} abuffer b {{{ RET (b, NONEV, bempty)%V; triple o (b, NONEV, bempty)%V }}}.
+  Proof.
+    iIntros (n o b Hn ψ) "Hb Hψ".
+    rewrite /abuffer /atriple_.
+    wp_pures.
+    iApply "Hψ".
+    rewrite triple_unfold.
+    iExists b, NONEV, bempty, o, [], [], n, 0, [].
+    iFrame.
+    iModIntro.
+    iSplitR. iPureIntro. constructor; list_elem_of.
+    repeat doneL.
+    iSplitL. rewrite isDeque_unfold. by iLeft.
+    iSplitL. by iApply bempty_spec.
+    repeat doneL.
+    iPureIntro. rewrite !app_nil_r //=.
+  Qed.
+
+  Lemma abuffer_spec : forall n o b,
+    n ∈ [2; 3] -> {{{ buffer n o b }}} abuffer b {{{ t, RET t; triple o t }}}.
+  Proof.
+    iIntros (n o k H ψ) "Hb Hψ".
+    wp_apply (abuffer_spec_explicit with "Hb") as "H". by assumption.
+    iApply "Hψ".
+    done.
+  Qed.
+
+
+End proofs.
