theories/eject_cost.v
@@ -1,0 +1,156 @@
+From iris.heap_lang Require Import lang proofmode notation.
+From iris.bi Require Import derived_laws.
+
+From Coq Require Import List.
+Import ListNotations.
+
+From AAC_tactics Require Import AAC.
+From AAC_tactics Require Import Instances.
+Import Instances.Lists.
+
+From Deque Require Import common tick shared_ref deque_cost eject_cost_lemmas.
+
+Section proof.
+
+  Context `{!heapGS Σ} `{!na_invG Σ}.
+  Context {π : gname}.
+
+  Lemma eject_spec_helper oD x (ℓ : loc) : forall depth,
+    {{{ isDeque π depth (oD ++ ⋅x) (SOMEV #ℓ) ∗ ⏱ time_for_pop ∗ Token π depth }}}
+      eject_nonempty (#ℓ)
+    {{{ d', RET (d', x)%V; isDeque π depth oD d' ∗ Token π depth }}}.
+  Proof.
+    Opaque isEjectFiveTuple isUnsafeEjectFiveTuple prepare_eject naive_eject.
+    iIntros (depth ψ) "(Hd & τ & O) Hψ".
+    rewrite isDeque_unfold.
+    rewrite /eject_nonempty.
+    Opaque eject_nonempty.
+    iLöb as "iH" forall (ℓ oD x depth ψ).
+    iDestruct "Hd" as "[[%H _] | (%ℓ' & %Heqℓ & Hℓ)]". by inversion H.
+    inversion Heqℓ as [H]. rewrite -H. clear Heqℓ H ℓ'.
+    wp_pures.
+    iDestruct (split_time 1 with "τ") as "[ι τ]". by lia.
+    wp_apply (tick_spec with "ι") as "_".
+    wp_pures.
+    wp_apply (ssref_load_open with "[Hℓ O]") as "%d (O & πd & DONE)".
+      { by iFrame. }
+    iDestruct (safe_decidable depth (oD++⋅x) d with "πd") as "[Unsafe | Safe]".
+    wp_pures.
+    2: {
+      wp_pures.
+      iDestruct "Safe" as (kp ks) "(Hsafe & τ' & eject_safe)".
+      iDestruct "Hsafe" as "#Hsafe".
+      gather_t "τ'".
+      iAssert (isPersFiveTuple π depth (oD ++ ⋅x) d) as "Hd".
+      - Transparent isEjectFiveTuple.
+        iDestruct "Hsafe" as "(%p & %l & %m & %r & %s & %op & %ol & %om & %or & %os &
+                            %kMd & %ltr & %rtr &
+                            -> & %conf & #Hp & #Hl & #Hm & #Hr & #Hs &
+                            #Hltr & #Hrtr & %Hoeq)".
+        Opaque isEjectFiveTuple.
+        iExists p, l, m, r, s, op, ol, om, or, os, kp, kMd, ks, ltr, rtr.
+        doneL.
+        iSplit. iPureIntro. inversion conf; by easy_config.
+        iFrame "#". iFrame.
+        done.
+      - wp_bind (naive_eject_safe d)%E.
+        iApply (wp_wand with "eject_safe").
+        iIntros (true_) "->".
+        Opaque isPersFiveTuple.
+        wp_pures.
+        iDestruct (split_time 3 with "τ") as "[ι τ]". by lia.
+        wp_bind (#ℓ <- d)%E.
+        iApply (wp_wand with "[DONE ι O Hd]").
+        {
+          iApply ("DONE" with "[ι Hd]"); [| by iFrame].
+          iNext.
+          iApply strutcure_and_time.
+          by iFrame.
+        }
+        iIntros (unit) "O".
+        wp_pures; clear unit.
+        wp_apply (safe_naive_eject with "[τ]") as (x' d' o') "(Hd' & %Heq)".
+          { iFrame "#".
+            split_t (kp ∘ ks); [| done].
+            destruct (buffer_colour (ks-1));
+            destruct (buffer_colour ks);
+            destruct (buffer_colour kp);
+            simpl; auto with arith.
+          }
+        destruct (app_sing_inv _ _ _ _ Heq) as [-> ->].
+        iApply "Hψ".
+        by iFrame.
+      Transparent isPersFiveTuple.
+    }
+    iDestruct "Unsafe" as "[Hunsafe eject_unsafe]".
+    wp_bind (naive_eject_safe d)%E.
+    iApply (wp_wand with "eject_unsafe").
+    iIntros (false_) "->".
+    wp_pures.
+    wp_apply (prepare_eject_spec with "[τ O Hunsafe]").
+    - iFrame.
+      iIntros (ℓ' x' o') "Hℓ' τ O".
+      Transparent eject_nonempty.
+      rewrite /eject_nonempty.
+      iApply ("iH" with "[Hℓ'] [τ] [O]"); iClear "iH"; try done.
+      + rewrite -isDeque_unfold. ℓisDeque ℓ'. iExact "Hℓ'".
+      + iNext.
+        iIntros (d') "[Hd O]".
+        iExists d'. iFrame. done.
+    - iIntros (f' kp ks) "(Hf' & O & τ)". iClear "iH".
+      wp_pures.
+      wp_bind (#ℓ <- f')%E.
+      Transparent isEjectFiveTuple.
+      iDestruct "Hf'" as "(%p & %l & %m & %r & %s & %op & %ol & %om & %or & %os &
+                          %kMd & %ltr & %rtr &
+                          -> & %conf & #Hp & #Hl & #Hm & #Hr & #Hs &
+                          #Hltr & #Hrtr & %Hoeq)".
+      split_t (kp ⋄ ks).
+      iApply (wp_wand with "[DONE O ι]").
+      {
+        iApply ("DONE" with "[ι]"); [| done].
+        iNext.
+        iExists p, l, m, r, s, op, ol, om, or, os, kp, kMd, ks, ltr, rtr.
+        doneL.
+        iSplit. iPureIntro. inversion conf; by easy_config.
+        iFrame "#". iFrame.
+        iSplit. iApply (big_sepL2_mono with "Hltr"). by auto.
+        iSplit. iApply (big_sepL2_mono with "Hrtr"). by auto.
+        done.
+      }
+      iIntros (unit) "O". wp_pures; clear unit.
+      wp_apply (safe_naive_eject with "[τ]").
+      + split_t (kp ∘ ks).
+        iFrame.
+        iExists p, l, m, r, s, op, ol, om, or, os, kMd, ltr, rtr.
+        doneL.
+        iSplit. iPureIntro. inversion conf; by easy_config.
+        iFrame "#". iFrame.
+        iSplit. iApply (big_sepL2_mono with "Hltr"). by auto.
+        iSplit. iApply (big_sepL2_mono with "Hrtr"). by auto.
+        done.
+      + iIntros (x' d' o') "[Hd %Heq]".
+        destruct (app_sing_inv _ _ _ _ Heq) as [-> ->].
+        iApply "Hψ".
+        iFrame.
+  Qed.
+
+  Definition eject_spec : forall x o d,
+    {{{ IsDeque π (o++⋅x) d ∗ Token π 0 ∗ ⏱ time_for_pop }}}
+      eject d
+    {{{ d', RET (d', x)%V; IsDeque π o d' ∗ Token π 0 }}}.
+  Proof.
+    iIntros (x o d ψ) "(#Hd & O & τ) hψ".
+    rewrite /eject.
+    wp_pures.
+    rewrite /IsDeque isDeque_unfold.
+    iCombine "Hd Hd" as "[_ [[-> %Heq]|(%ℓ & -> & Hℓ)]]";
+      rewrite -isDeque_unfold;
+      [ destruct o; simpl in Heq; inversion Heq |].
+    wp_pures.
+    wp_apply (eject_spec_helper with "[O τ]").
+      by (iFrame; iFrame "#").
+    done.
+  Qed.
+
+End proof.
