theories/eject_cost_lemmas.v
@@ -1,0 +1,1550 @@
+From iris.heap_lang Require Import lang proofmode notation.
+From iris.bi Require Import derived_laws.
+
+From Coq Require Import List.
+Import ListNotations.
+
+From AAC_tactics Require Import AAC.
+From AAC_tactics Require Import Instances.
+Import Instances.Lists.
+
+From Deque Require Import common tick shared_ref deque_cost push_cost concat_cost pop_cost_lemmas.
+
+Section lemmas.
+
+  Context `{!heapGS Σ} `{!na_invG Σ}.
+  Context {π : gname}.
+
+  Notation "kp ∘ ks" := (kp ⋄ ks - 1).
+  Definition Δ (kp ks : nat) := (kp ∘ ks) - (kp ⋄ ks).
+  Notation "kp ⊻ ks" := ((kp ∘ ks) + (kp ⋄ ks)) (at level 60).
+
+  (* Five-tuple configuration for calling naive_eject *)
+  Inductive eject_configuration : nat -> nat -> nat -> nat -> nat -> Prop :=
+    | eject_suffix_only : forall s, s ∈ [1..8] -> eject_configuration 0 0 0 0 s
+    | eject_has_middle : forall p ld rd s, p ∈ [3..6] -> s ∈ [4..6] -> eject_configuration p ld 2 rd s.
+
+ Definition isEjectFiveTuple := (
+    λ n o kPr kSf d, ∃ (pr ld md rd sf : val)
+      pr_content left_content md_content right_content sf_content
+      (kMd : nat) left_triples right_triples,
+      ⌜ d = (pr, ld, md, rd, sf)%V ⌝ ∗
+      ⌜ eject_configuration kPr (length left_content) kMd (length right_content) kSf ⌝ ∗
+      buffer kPr pr_content pr ∗
+      isDeque π (S n) left_triples ld ∗
+      buffer kMd md_content md ∗
+      isDeque π (S n) right_triples rd ∗
+      buffer kSf sf_content sf ∗
+      ([∗list] c;tr ∈ left_content;left_triples, ▷ triple π (S n) c tr) ∗
+      ([∗list] c;tr ∈ right_content;right_triples, ▷ triple π (S n) c tr) ∗
+      ⌜ o = pr_content ++ List.concat left_content ++ md_content ++ List.concat right_content ++ sf_content ⌝
+  )%I.
+
+ Definition isUnsafeEjectFiveTuple := (
+    λ π n o d, ∃ (pr ld md rd sf : val)
+      pr_content left_content md_content right_content sf_content
+      (kPr : nat) left_triples right_triples,
+      ⌜ d = (pr, ld, md, rd, sf)%V ⌝ ∗
+      ⌜ five_tuple_configuration kPr (length left_content) 2 (length right_content) 3 ⌝ ∗
+      five_tuple_potential kPr 3 ∗
+      buffer kPr pr_content pr ∗
+      isDeque π (S n) left_triples ld ∗
+      buffer 2 md_content md ∗
+      isDeque π (S n) right_triples rd ∗
+      buffer 3 sf_content sf ∗
+      ([∗list] c;tr ∈ left_content;left_triples, ▷ triple π (S n) c tr) ∗
+      ([∗list] c;tr ∈ right_content;right_triples, ▷ triple π (S n) c tr) ∗
+      ⌜ o = pr_content ++ List.concat left_content ++ md_content ++ List.concat right_content ++ sf_content ⌝
+  )%I.
+
+  Lemma safe_decidable : forall n o f,
+    fiveTuple π n o f -∗
+      (isUnsafeEjectFiveTuple π n o f ∗ WP naive_eject_safe f {{ x, ⌜ x = #false ⌝ }})
+    ∨ ∃ kp ks, isEjectFiveTuple n o kp ks f ∗ ⏱ (kp ⋄ ks) ∗ WP naive_eject_safe f {{ x, ⌜ x = #true ⌝ }}.
+  Proof.
+    iIntros (n o f) "(%p & %l & %m & %r & %s & %op & %ol & %om & %or & %os &
+                      %kPr & %kMd & %kSf & %ltr & %rtr &
+                      %Heq & %conf & pot & #Hp & #Hl & #Hm & #Hr & #Hs &
+                      #Hltr & #Hrtr & %Hoeq)".
+    inversion conf.
+    - iRight.
+      iExists 0, kSf.
+      iFrame.
+      iSplitL.
+      + iExists p, l, m, r, s, op, ol, om, or, os, 0, ltr, rtr.
+        iFrame "#".
+        doneL.
+        iSplit. iPureIntro. rewrite -H -H1. by easy_config.
+        done.
+      + rewrite /naive_eject_safe.
+        rewrite Heq.
+        wp_pures.
+        wp_apply (bis_empty_spec with "Hm") as "_".
+        wp_pures.
+        done.
+    - destruct (dec_eq_nat kSf 3) as [-> | HkSf]; [iLeft | iRight].
+      + iSplitL.
+        * iExists p, l, m, r, s, op, ol, om, or, os, kPr, ltr, rtr.
+          iFrame "#". iFrame.
+          doneL.
+          rewrite {3}H3.
+          iSplit; done.
+        * rewrite /naive_eject_safe Heq.
+          wp_pures.
+          wp_apply (bis_empty_spec with "Hm") as "_".
+          wp_pures.
+          wp_apply (blength_spec with "Hs") as "_".
+          wp_pures.
+          done.
+      + iExists kPr, kSf. iSplitR.
+        * iExists p, l, m, r, s, op, ol, om, or, os, kMd, ltr, rtr.
+          rewrite -H3.
+          iFrame. iFrame "#".
+          doneL.
+          iSplit. iPureIntro. apply eject_has_middle; invert_all_in.
+          done.
+        * rewrite /naive_eject_safe Heq.
+          iFrame.
+          wp_pures.
+          wp_apply (bis_empty_spec with "Hm") as "_".
+          wp_pures.
+          wp_apply (blength_spec with "Hs") as "_".
+          invert_all_in; wp_pures; done.
+  Qed.
+
+  Ltac suffix_only_incantation op om H H1 Hoeq :=
+    iDestruct (buffer_length with "Hp") as "%LprC";
+    destruct op; [| inversion LprC];
+    iDestruct (buffer_length with "Hm") as "%LmdC";
+    destruct om; [| inversion LmdC];
+    symmetry in H; rewrite (nil_length_inv _ H) in Hoeq |- *;
+    symmetry in H1; rewrite (nil_length_inv _ H1) in Hoeq |- *;
+    iDestruct (big_sepL2_nil_inv_l with "Hltr") as "->";
+    iDestruct (big_sepL2_nil_inv_l with "Hrtr") as "->".
+
+  Ltac split_t τ := iDestruct (split_time τ with "τ") as "[ι τ]"; [ try lia |].
+  Ltac split_ti kp ks := iDestruct (split_time (kp ⊻ ks) with "τ") as "[ι τ]"; [ invert_all_in; simpl; try lia |].
+  Ltac split_Δ kp ks := split_t (Z.to_nat (Δ kp ks)); [ try (invert_all_in; rewrite /Δ /=; lia) |].
+  Ltac gather_t pot := iDestruct (time_combine with String.concat "" ["[τ "; pot; "]"]) as "τ"; [ iFrame |].
+
+  Lemma safe_naive_eject : forall n o kp ks f,
+    {{{ isEjectFiveTuple n o kp ks f ∗ ⏱ (kp ∘ ks) }}}
+      naive_eject f
+    {{{ x d o', RET (d, x)%V; isDeque π n o' d ∗ ⌜ o = o' ++ ⋅x ⌝ }}}.
+  Proof.
+    iIntros (n o kPr kSf f ψ) "[Hf τ] Hψ".
+    iDestruct "Hf" as "(%p & %l & %m & %r & %s & %op & %ol & %om & %or & %os &
+                      %kMd & %ltr & %rtr &
+                      -> & %conf & #Hp & #Hl & #Hm & #Hr & #Hs &
+                      #Hltr & #Hrtr & %Hoeq)".
+    rewrite /naive_eject.
+    wp_pures.
+    inversion conf; wp_pures.
+    - suffix_only_incantation op om H H1 Hoeq.
+      change (kSf ∈ map S [0;1;2;3;4;5;6;7]) in H3.
+      assert (∃ kSf', kSf = kSf' + 1) as (kSf' & ->)
+        by (invert_all_in;
+        match goal with
+        | |- ∃ kSf', S ?x = kSf' + 1 => exists x; lia
+        end).
+      wp_apply (beject_spec with "Hs") as "%b' %o' %x (#Hb & ->)".
+      rewrite /assemble /assemble_.
+      wp_pures.
+      wp_apply (bis_empty_spec with "Hm") as "_". wp_pures.
+      wp_apply (bis_empty_spec with "Hb") as "_".
+      destruct kSf'; wp_pures.
+      + iApply "Hψ".
+        iDestruct (buffer_length with "Hb") as "%LbC".
+        destruct o'; [| inversion LbC].
+        iModIntro.
+        iSplit.
+        * by isEmptyDeque.
+        * iPureIntro.
+          rewrite Hoeq //.
+      + wp_bind (ref _)%E.
+        wp_apply (ssref_alloc π (fiveTuple π n o') with "[τ]") as "%ℓ'' #Hℓ''".
+        * iExists p,l,m,r,b',[],[],[],[],o',0,0,(S kSf'),[],[].
+          rewrite /concat !app_nil_l in Hoeq.
+          iFrame. iFrame "#".
+          doneL.
+          assert (S kSf' ∈ [1..7]).
+            { assert (S kSf' + 1 = S (S kSf')) as Heq by lia.
+              rewrite Heq in H3.
+              invert_all_in; list_elem_of.
+            }
+          clear H3.
+          iSplit. iPureIntro. by constructor; invert_all_in; list_elem_of.
+          iSplit. rewrite /five_tuple_potential /=.
+            iDestruct (split_time (0 ⋄ S kSf') with "τ") as "[ι _]".
+              { invert_all_in; auto with arith. }
+            iExact "ι".
+          do 2 doneL.
+          iPureIntro.
+          rewrite //.
+        * wp_pures.
+          iModIntro.
+          iApply "Hψ".
+          iSplit. by ℓisDeque ℓ''.
+          iPureIntro. rewrite Hoeq //.
+    - change (kSf ∈ map S [3;4;5]) in H0.
+      apply decrease_in in H0 as (kS & -> & H0).
+      wp_apply (beject_spec with "Hs") as "%b' %o' %x (#Hb' & ->)".
+      rewrite /assemble.
+      wp_pures.
+      split_t (kPr ⋄ kS). by invert_all_in.
+      wp_apply (bis_empty_spec with "Hm") as "_".
+      rewrite /assemble_.
+      wp_pures.
+      wp_apply (ssref_alloc π (fiveTuple π n _) with "[ι]") as "%ℓ'' #Hℓ''".
+      + iExists p,l,m,r,b',op,ol,om,or,o',kPr,kMd,kS,ltr,rtr.
+        rewrite -H3.
+        iFrame. iFrame "#".
+        doneL.
+        iSplit. iPureIntro. by constructor; invert_all_in; list_elem_of.
+        iSplit. iApply (big_sepL2_mono with "Hltr"). by auto.
+        iSplit. iApply (big_sepL2_mono with "Hrtr"). by auto.
+        done.
+      + wp_pures.
+        iModIntro.
+        iApply "Hψ".
+        iSplit. by ℓisDeque ℓ''.
+        iPureIntro. rewrite Hoeq. aac_reflexivity.
+  Qed.
+
+  Lemma unsafe_naive_eject : forall n o f,
+    {{{ fiveTuple π n o f ∗ ⏱ 1 }}}
+      naive_eject f
+    {{{ x (d : val) o', RET (d, x)%V;
+      ⌜ o = o' ++ ⋅x ⌝ ∗
+      ∀ y : val,
+        WP inject d y {{ d, isDeque π n (o' ++ ⋅y) d }}
+    }}}.
+  Proof.
+    iIntros (n o f ψ) "[Hf τ] Hψ".
+    iDestruct "Hf" as "(%p & %l & %m & %r & %s & %op & %ol & %om & %or & %os &
+                      %kPr & %kMd & %kSf & %ltr & %rtr &
+                      -> & %conf & pot & #Hp & #Hl & #Hm & #Hr & #Hs &
+                      #Hltr & #Hrtr & %Hoeq)".
+    rewrite /naive_eject.
+    wp_pures.
+    inversion conf; wp_pures.
+    - suffix_only_incantation op om H H1 Hoeq.
+      iClear "Hl Hr".
+      change (kSf ∈ map S [0;1;2;3;4;5;6;7]) in H3.
+      apply decrease_in in H3 as (ks & -> & Hks).
+      wp_apply (beject_spec with "Hs") as (b' o' x) "[#Hb' %Hoeq']".
+      rewrite /assemble.
+      wp_pures.
+      wp_apply (bis_empty_spec with "Hm") as "_".
+      wp_pures.
+      wp_apply (bis_empty_spec with "Hb'") as "_".
+      inversion Hks; wp_pures.
+      + iApply "Hψ".
+        iModIntro.
+        iSplit.
+        * iPureIntro.
+          aac_rewrite Hoeq.
+          rewrite //.
+        * iIntros (y).
+          rewrite /inject.
+          wp_pures.
+          wp_apply (tick_spec with "τ") as "_".
+          rewrite /asingleton.
+          wp_pures.
+          wp_apply (bpush_spec) as (b) "Hb". by iApply bempty_spec.
+          wp_pures.
+          wp_apply (ssref_alloc _ (fiveTuple π n [y]) with "[Hb]") as (ℓ) "Hℓ".
+            { iExists bempty, NONEV, bempty, NONEV, b, [], [], [], [], [y], 0, 0, 1, [], [].
+              rewrite !app_nil_r /five_tuple_potential /=.
+              iFrame. iFrame "#".
+              repeat doneL.
+              iSplit. by easy_config.
+              iSplit. by iApply time_zero.
+              repeat (iSplit; [iApply bempty_spec || isEmptyDeque |]).
+              done.
+            }
+          wp_pures.
+          iModIntro.
+          rewrite /=.
+          iDestruct (buffer_length with "Hs") as "%Hos".
+          destruct os; [inversion Hos |].
+          destruct os; [| inversion Hos].
+          destruct o'; [| inversion Hoeq'].
+          -- ℓisDeque ℓ.
+            iExact "Hℓ".
+          -- exfalso.
+            symmetry in H9.
+            apply app_nil_r_inv in H9.
+            inversion H9.
+      + clear Hks.
+        assert (bool_decide (ks = 0%nat) = false) as -> by invert_all_in.
+        rewrite /assemble_.
+        wp_pures.
+        wp_alloc ℓ as "Hℓ".
+        wp_pures.
+        iModIntro.
+        iApply "Hψ".
+        iSplit. iPureIntro; aac_rewrite Hoeq; by rewrite //.
+        iIntros (y').
+        rewrite /inject.
+        wp_pures.
+        wp_apply (tick_spec with "τ") as "_".
+        wp_pures.
+        wp_load.
+        wp_pures.
+        wp_apply (bis_empty_spec with "Hm") as "_".
+        wp_pures.
+        wp_apply (bhas_length_8_spec with "Hb'") as "_".
+        assert (bool_decide (ks = 8%nat) = false) as -> by invert_all_in.
+        wp_pures.
+        wp_store.
+        rewrite /assemble_.
+        wp_apply (binject_spec with "Hb'") as (b) "Hb".
+        wp_pures.
+        wp_apply (ssref_alloc _ (fiveTuple π n (o' ++ ⋅y')) with "[Hb pot]") as (ℓ') "Hℓ'".
+          { iExists bempty, NONEV, bempty, NONEV, b, [], [], [], [], (o'++⋅y'), 0, 0, (ks+1), [], [].
+            rewrite /five_tuple_potential /=.
+            iFrame. iFrame "#".
+            repeat doneL.
+            iSplit. rewrite H H1 -H0 -H2 in conf. done.
+            repeat (iSplit; [iApply bempty_spec || isEmptyDeque |]).
+            done.
+          }
+        wp_pures.
+        iModIntro.
+        rewrite /=.
+        ℓisDeque ℓ'.
+        iExact "Hℓ'".
+    - change (kSf ∈ map S [2; 3; 4; 5]) in H0.
+      apply decrease_in in H0 as (ks & -> & Hks).
+      wp_apply (beject_spec with "Hs") as "%b' %o' %x (#Hb' & ->)".
+      rewrite /assemble.
+      wp_pures.
+      wp_apply (bis_empty_spec with "Hm") as "_".
+      rewrite /assemble_.
+      wp_pures.
+      wp_alloc ℓ as "Hℓ".
+      wp_pures.
+      iModIntro.
+      iApply ("Hψ" $! x (SOMEV #ℓ) (op ++ concat ol ++ om ++ concat or ++ o')).
+      iSplit. iPureIntro. rewrite Hoeq. aac_reflexivity.
+      iIntros (y).
+      rewrite /inject.
+      wp_pures.
+      wp_apply (tick_spec with "τ") as "_".
+      wp_pures.
+      wp_load.
+      wp_pures.
+      wp_apply (bis_empty_spec with "Hm") as "_".
+      wp_pures.
+      wp_apply (bhas_length_6_spec with "Hb'") as "_".
+      assert (bool_decide (ks = 6%nat) = false) as  -> by invert_all_in.
+      wp_pures.
+      wp_store.
+      rewrite /assemble_.
+      wp_apply (binject_spec with "Hb'") as "%p' #Hp'".
+      wp_pures.
+      wp_apply (ssref_alloc π (fiveTuple π n (op ++ concat ol ++ om ++ concat or ++ o' ++ ⋅y)) with "[pot]") as "%ℓ' Hℓ'".
+      + iExists p,l,m,r,p',op,ol,om,or,(o'++⋅y),kPr,2,(ks+1),ltr,rtr.
+        iFrame "#".
+        doneL.
+        iSplit. iPureIntro. rewrite H3. done.
+        iSplit. iExact "pot".
+        iSplit. iApply (big_sepL2_mono with "Hltr"). by auto.
+        iSplit. iApply (big_sepL2_mono with "Hrtr"). by auto.
+        done.
+      + wp_pures.
+        iModIntro.
+        rewrite -!app_assoc.
+        ℓisDeque ℓ'.
+        iExact "Hℓ'".
+  Qed.
+
+  Lemma destruct_end {A} : forall (θ : list A),
+    θ = [] ∨ ∃ θ' e, θ = θ' ++ ⋅e.
+  Proof.
+    induction θ.
+    - by left.
+    - assert (a :: θ = ⋅a ++ θ) as -> by reflexivity.
+      right.
+      destruct IHθ as [-> | (o & e & ->)].
+      + by exists [], a.
+      + by exists (⋅a++o), e.
+  Qed.
+
+  Lemma inspect_last_spec : forall n o f,
+    {{{ isPersFiveTuple π n o f }}}
+      inspect_last f
+    {{{ o' t, RET t; ⌜ o = o' ++ ⋅t ⌝  }}}.
+  Proof.
+    iIntros (n o f ψ) "Hf Hψ".
+    iDestruct "Hf" as "(%p & %l & %m & %r & %s & %op & %ol & %om & %or & %os &
+                      %kPr & %kMd & %kSf & %ltr & %rtr &
+                      -> & %conf & #Hp & #Hl & #Hm & #Hr & #Hs &
+                      #Hltr & #Hrtr & %Hoeq)".
+    rewrite /inspect_last. wp_pures.
+    inversion conf; wp_pures.
+    - change (kSf ∈ map S [0;1;2;3;4;5;6;7]) in H3.
+      apply decrease_in in H3 as (kS & -> & HkS).
+      destruct (destruct_end os) as [-> | (os' & x & ->)].
+        { iDestruct (buffer_length with "Hs") as "%abs".
+          simpl in abs; lia. }
+      wp_apply (blast_spec with "Hs") as "_".
+      iApply "Hψ".
+      suffix_only_incantation op om H H1 Hoeq.
+      iPureIntro.
+      rewrite Hoeq //.
+    - change (kSf ∈ map S [2;3;4;5]) in H0.
+      apply decrease_in in H0 as (kS & -> & HkS).
+      destruct (destruct_end os) as [-> | (os' & x & ->)].
+        { iDestruct (buffer_length with "Hs") as "%abs".
+          simpl in abs; lia. }
+      wp_apply (blast_spec with "Hs") as "_".
+      iApply "Hψ".
+      iPureIntro.
+      rewrite Hoeq !app_assoc //.
+  Qed.
+
+  Inductive special_triple_configuration : nat -> nat -> nat -> Prop :=
+    | is_special_three : forall x, x ∈ [0; 2; 3] -> special_triple_configuration x 0 3
+    | is_special_child : forall x o y, x ∈ [2; 3] -> o > 0 -> y ∈ [2; 3] -> special_triple_configuration x o y
+    | is_special_first : forall x o y, x ∈ [2; 3] -> y ∈ [2; 3] -> special_triple_configuration x o y.
+
+  Inductive not_special_triple_configuration : nat -> nat -> nat -> Prop :=
+    | is_bad : not_special_triple_configuration 0 0 2.
+
+  Definition isSpecialTriple := (
+    λ n o t,
+      ∃ (fst ch lst : val)
+        fst_content child_content lst_content
+        (kFst kLst : nat) triples,
+        ⌜ special_triple_configuration kFst (length child_content) kLst ⌝ ∗
+        ⌜ t = (fst, ch, lst)%V ⌝ ∗
+        buffer kFst fst_content fst ∗
+        isDeque π n triples ch ∗
+        buffer kLst lst_content lst ∗
+        ([∗list] c;tr ∈ child_content;triples, ▷ triple π n c tr) ∗
+        ⌜ o = fst_content ++ List.concat child_content ++ lst_content ⌝
+  )%I.
+
+  Definition isNotSpecialTriple := (
+    λ n o t,
+      ∃ (fst ch lst : val)
+        fst_content child_content lst_content
+        (kFst kLst : nat) triples,
+        ⌜ not_special_triple_configuration kFst (length child_content) kLst ⌝ ∗
+        ⌜ t = (fst, ch, lst)%V ⌝ ∗
+        buffer kFst fst_content fst ∗
+        isDeque π n triples ch ∗
+        buffer kLst lst_content lst ∗
+        ([∗list] c;tr ∈ child_content;triples, ▷ triple π n c tr) ∗
+        ⌜ o = fst_content ++ List.concat child_content ++ lst_content ⌝
+  )%I.
+
+  (* NOTE(Juliette): slightly different: antinormalisation is necessary to have the right format for analysis *)
+  (*
+  Lemma special_decidable : forall n o t,
+    triple π n o t -∗
+    WP antinormalize t {{ t',
+      isSpecialTriple n o t'
+    ∨ isNotSpecialTriple n o t'
+    }}.
+  Proof.
+    iIntros (n o t) "Ht".
+    rewrite triple_unfold.
+    iDestruct "Ht" as (f c l fc cc lc kFst kLst tr) "(%conf & -> & #Hf & #Hc & #Hl & Htr & %Hoeq)".
+    rewrite /antinormalize; wp_pures.
+    inversion conf.
+    - inversion H2.
+      + inversion H0; wp_apply (bis_empty_spec with "Hl") as "_"; wp_pures.
+        * iRight.
+          iDestruct (buffer_length with "Hl") as "%H'".
+          destruct lc; [| inversion H'].
+          destruct cc; [| inversion H].
+          iDestruct (big_sepL2_nil_inv_l with "Htr") as "->".
+          iExists bempty, c, f, [], [], fc, 0, kFst, [].
+          rewrite H9.
+          iFrame. iFrame "#".
+          iSplitR. iPureIntro. rewrite -H. by constructor.
+          doneL.
+          iSplitR. by iApply bempty_spec.
+          iSplitR. iModIntro. done.
+          iPureIntro.
+          rewrite Hoeq /= app_nil_r //.
+        * inversion H9; [| inversion H13 ].
+          iLeft.
+          iDestruct (buffer_length with "Hl") as "%H'".
+          destruct lc; [| inversion H'].
+          destruct cc; [| inversion H].
+          iDestruct (big_sepL2_nil_inv_l with "Htr") as "->".
+          iExists bempty, c, f, [], [], fc, 0, kFst, [].
+          rewrite H13.
+          iFrame "#".
+          iSplitR. iPureIntro. simpl. by easy_config.
+          doneL.
+          iSplitR. by iApply bempty_spec.
+          iSplitR. iModIntro. done.
+          iPureIntro.
+          rewrite Hoeq /= app_nil_r //.
+      + wp_apply (bis_empty_spec with "Hl") as "_"; wp_pures.
+        clear l0 H7 H2 H3 x0 y0 H4 H5.
+        assert (bool_decide (kLst = 0%nat) = false) as -> by invert_all_in.
+        wp_pures.
+        iLeft. iModIntro.
+        destruct cc; [| inversion H].
+        iDestruct (big_sepL2_nil_inv_l with "Htr") as "->".
+        iExists f, c, l, fc, [], lc, kFst, kLst, [].
+        iFrame "#".
+        iSplitR. iPureIntro. simpl. by easy_config.
+        doneL.
+        doneL.
+        done.
+    - wp_apply (bis_empty_spec with "Hl") as "_".
+      assert (bool_decide (kLst = 0%nat) = false) as -> by invert_all_in.
+      wp_pures.
+      iLeft. iModIntro.
+      iExists f, c, l, fc, cc, lc, kFst, kLst, tr.
+      iFrame "#".
+      iSplitR. iPureIntro. simpl. by easy_config.
+      doneL.
+      doneR.
+      iApply (big_sepL2_mono with "Htr"). by auto.
+  Qed.
+  *)
+  Lemma antinormalize_special_spec : forall n o t,
+    {{{ @pop_cost_lemmas.isSpecialTriple Σ _ _ π  n o t }}}
+      antinormalize t
+    {{{ t', RET t'; isSpecialTriple n o t' }}}.
+  Proof.
+    iIntros (n o t ψ) "Ht Hψ".
+    iDestruct "Ht" as (f c l fc cc lc kFst kLst tr) "(%conf & -> & #Hf & #Hc & #Hl & Htr & %Hoeq)".
+    rewrite /antinormalize.
+    inversion conf; wp_pures; wp_apply (bis_empty_spec with "Hl") as "_"; wp_pures.
+    - inversion H1.
+      + wp_pures.
+        iApply "Hψ". iModIntro.
+        iDestruct (buffer_length with "Hl") as "%H'".
+        destruct lc; [| inversion H'].
+        destruct cc; [| inversion H].
+        iDestruct (big_sepL2_nil_inv_l with "Htr") as "->".
+        iExists bempty, c, f, [], [], fc, 0, kFst, [].
+        rewrite -H0.
+        iFrame "#".
+        iSplitR. iPureIntro. simpl. by easy_config.
+        doneL.
+        iSplitR. by iApply bempty_spec.
+        doneL.
+        iPureIntro.
+        rewrite Hoeq /= app_nil_r //.
+      + assert (bool_decide (kLst = 0%nat) = false) as -> by invert_all_in.
+        wp_pures.
+        iApply "Hψ". iModIntro.
+        destruct cc; [| inversion H].
+        iDestruct (big_sepL2_nil_inv_l with "Htr") as "->".
+        iExists f, c, l, fc, [], lc, kFst, kLst, [].
+        rewrite -H0.
+        iFrame "#".
+        iSplitR. iPureIntro. simpl. by easy_config.
+        doneL.
+        doneL.
+        done.
+    - assert (bool_decide (kLst = 0%nat) = false) as -> by invert_all_in.
+      wp_pures.
+      iApply "Hψ". iModIntro.
+      iExists f, c, l, fc, cc, lc, kFst, kLst, tr.
+      iFrame "#".
+      iSplitR. iPureIntro. simpl. by easy_config.
+      doneL.
+      iSplitL. iApply (big_sepL2_mono with "Htr"). by auto.
+      done.
+    - assert (bool_decide (kLst = 0%nat) = false) as -> by invert_all_in.
+      wp_pures.
+      iApply "Hψ". iModIntro.
+      iExists f, c, l, fc, cc, lc, kFst, kLst, tr.
+      iFrame "#".
+      iSplitR. iPureIntro. simpl. by easy_config.
+      doneL.
+      iSplitL. iApply (big_sepL2_mono with "Htr"). by auto.
+      done.
+  Qed.
+
+  Lemma antinormalize_not_special_spec : forall n o t,
+    {{{ @pop_cost_lemmas.isNotSpecialTriple Σ _ _ π n o t }}}
+      antinormalize t
+    {{{ t', RET t'; isNotSpecialTriple n o t' }}}.
+  Proof.
+    iIntros (n o t ψ) "Ht Hψ".
+    iDestruct "Ht" as (f c l fc cc lc kFst kLst tr) "(%conf & -> & #Hf & #Hc & #Hl & Htr & %Hoeq)".
+    rewrite /antinormalize.
+    inversion conf; wp_pures; wp_apply (bis_empty_spec with "Hl") as "_"; wp_pures.
+    iModIntro.
+    iApply "Hψ".
+    iDestruct (buffer_length with "Hl") as "%H'".
+    destruct lc; [| inversion H'].
+    destruct cc; [| inversion H1].
+    iDestruct (big_sepL2_nil_inv_l with "Htr") as "->".
+    iExists bempty, c, f, [], [], fc, 0, kFst, [].
+    rewrite -H.
+    iFrame "#".
+    iSplitR. iPureIntro. simpl. by easy_config.
+    doneL.
+    iSplitR. by iApply bempty_spec.
+    doneL.
+    iPureIntro.
+    rewrite Hoeq /= app_nil_r //.
+  Qed.
+
+  Definition isPersFiveTupleLaterRemoved := (
+    λ n o d, ∃ (pr ld md rd sf : val)
+      pr_content left_content md_content right_content sf_content
+      (kPr kMd kSf : nat) left_triples right_triples,
+      ⌜ d = (pr, ld, md, rd, sf)%V ⌝ ∗
+      ⌜ five_tuple_configuration kPr (length left_content) kMd (length right_content) kSf ⌝ ∗
+      buffer kPr pr_content pr ∗
+      isDeque π (S n) left_triples ld ∗
+      buffer kMd md_content md ∗
+      isDeque π (S n) right_triples rd ∗
+      buffer kSf sf_content sf ∗
+      ([∗list] c;tr ∈ left_content;left_triples, triple π (S n) c tr) ∗
+      ([∗list] c;tr ∈ right_content;right_triples, triple π (S n) c tr) ∗
+      ⌜ o = pr_content ++ List.concat left_content ++ md_content ++ List.concat right_content ++ sf_content ⌝
+  )%I.
+
+  Lemma add_later : forall n o d, isPersFiveTupleLaterRemoved n o d -∗ isPersFiveTuple π n o d.
+  Proof.
+    iIntros (n o d) "Hd".
+    iDestruct "Hd" as (p l m r s op ol om or os kp km ks ltr rtr)
+      "(-> & conf & hp & hl & hm & hr & hs & hltr & hrtr & heq)".
+    iExists p, l, m, r, s, op, ol, om, or, os, kp, km, ks, ltr, rtr.
+    iFrame.
+    doneL.
+    iSplitL "hltr".
+    - iApply (big_sepL2_mono with "hltr"). by auto.
+    - iApply (big_sepL2_mono with "hrtr"). by auto.
+  Qed.
+
+  Lemma app_sing_inv {A} : forall (o o' : list A) (x y : A),
+    o ++ ⋅x = o' ++ ⋅y -> o = o' ∧ x = y.
+  Proof.
+    induction o; intros.
+    - rewrite app_nil_l in H.
+      apply (f_equal length) in H as H'.
+      rewrite length_app /= in H'.
+      assert (length o' = 0) by lia.
+      destruct o'.
+      + by inversion H.
+      + simpl in H0. lia.
+    - destruct o'. inversion H.
+      + apply (f_equal length) in H2.
+        rewrite length_app /= in H2.
+        lia.
+      + rewrite -!app_comm_cons in H.
+        inversion H.
+        by specialize (IHo o' x y H2) as [-> ->].
+  Qed.
+
+  Lemma eject_triple_spec : forall n os tr ℓ,
+    {{{ ℓ ⤇{π, n} fiveTuple π n tr ∗ Token π n
+      ∗ ⏱ time_for_pop ∗ ([∗list] x;y ∈ os;tr, triple π n x y)
+      ∗ (∀ ℓ x o,
+          ℓ ⤇{π, n} fiveTuple π n (o ++ ⋅x) -∗
+          ⏱ time_for_pop -∗
+          Token π n -∗
+          WP eject_nonempty #ℓ
+            {{ r, ∃ d, ⌜ r = (d, x)%V ⌝ ∗ isDeque π n o d ∗ Token π n }})
+    }}}
+      subst "eject_nonempty" eject_nonempty (eject_triple #ℓ)
+    {{{ t' t o tr' os' (d' : val), RET (d', t)%V; Token π n ∗
+      ⌜ tr = tr' ++ ⋅t' ∧ os = os' ++ ⋅o ⌝ ∗
+      ([∗list] x;y ∈ os';tr', triple π n x y) ∗
+      ( isSpecialTriple n o t ∗ ⏱ (time_for_pop-4) ∗ (∀ x : val, WP inject d' x {{ d'', isDeque π n (tr' ++ ⋅x) d'' }})
+      ∨ isNotSpecialTriple n o t ∗ isDeque π n tr' d'
+      )
+    }}}.
+  Proof.
+    iIntros (n os tr d Hψ) "(#Hd & O & τ & Htr & iH) Hψ".
+    rewrite /pop_triple.
+    wp_pures.
+    wp_apply (ssref_read _ _ _ with "[O]").
+    { iFrame "#". iFrame.
+      iIntros (v) "Hv".
+      by iApply persist_structure.
+    }
+    Opaque isPersFiveTuple.
+    iIntros (f) "[#Hf O]".
+    wp_pures.
+    wp_apply (inspect_last_spec with "[Hf]").
+      { iExact "Hf". }
+    iIntros (o t) "->".
+    wp_pures.
+    destruct (destruct_end os) as [-> | (os' & l &  ->)].
+      iDestruct (big_sepL2_nil_inv_l with "Htr") as "%No".
+        apply app_nil_r_inv in No.
+        inversion No.
+    rename os' into os.
+    iDestruct (big_sepL2_app_inv with "Htr") as "(Htr & Ht)". by right.
+    iAssert (triple π n l t) with "[Ht]" as "Ht".
+      { simpl. iDestruct "Ht" as "[A _]". done. }
+    iDestruct (pop_cost_lemmas.special_decidable with "Ht") as "[#Ht' | #Ht']";
+    iCombine "Ht' Ht'" as "[Ht! Ht!']";
+    iDestruct "Ht!'" as (fi c la fc cc lc kF kL tr) "(%conf & -> & Hf' & Hc & Hl & Htrtr & %Hleq)";
+    inversion conf.
+    Opaque pop_cost_lemmas.isSpecialTriple pop_cost_lemmas.isNotSpecialTriple isSpecialTriple isNotSpecialTriple.
+    + rewrite isDeque_unfold.
+      iDestruct "Hc" as "[[-> ->] | (%ℓ & -> & Hℓ)]".
+      2: {
+        iDestruct (na_own_acc (↑ W n) with "O") as "[O A]". by apply access_stage.
+        iInv "Hℓ" as "[(%v' & Hv' & Hℓ') O]".
+        wp_pure.
+        iExFalso.
+        iDestruct "Hv'" as (pr' ld' md' rd' sf' pc' lc' mc' rc' sc' kp' km' ks' lt rt) "(_ & %conf' & _ & _ & _ & _ & _ & Hs & _ & _ & ->)".
+        iDestruct (big_sepL2_length with "Htrtr") as "%Hlen".
+        rewrite Hlen in H.
+        iDestruct (buffer_length with "Hs") as "%Hslen".
+        assert (ks' > 0) as Hslen' by (inversion conf'; invert_all_in; lia).
+        rewrite !length_app in H.
+        lia.
+      }
+      wp_pures.
+      iDestruct (split_time 1 with "τ") as "[ι τ]". by lia.
+      iDestruct (split_time 3 with "τ") as "[ι' τ]". by lia.
+      wp_apply (bhas_length_3_spec with "Hf'") as "_".
+      wp_pures.
+      wp_apply (unsafe_naive_eject with "[ι ι']").
+        { iFrame.
+          iDestruct (strutcure_and_time with "[ι']") as "H".
+            { iFrame.
+              by iExact "Hf". }
+          iExact "H". }
+      iIntros (x' d' o') "(%Hoeq' & Hpush)".
+      wp_pures.
+      apply app_sing_inv in Hoeq' as [-> <-].
+      wp_apply (antinormalize_special_spec with "Ht!") as (t') "Ht''".
+      wp_pures. iModIntro.
+      iApply "Hψ".
+      iSplitL "O". done.
+      doneL.
+      iSplit. iExact "Htr".
+      iLeft.
+      iSplitL "Ht''"; [| iSplitL "τ"].
+      * iExact "Ht''".
+      * by iDestruct (split_time (time_for_pop - 4) with "[τ]") as "[ι _]".
+      * iExact "Hpush".
+    + (* NOTE(Juliette): dedup *)
+      wp_pures.
+      rewrite isDeque_unfold.
+      iDestruct "Hc" as "[[-> ->] | (%ℓ & -> & Hℓ)]".
+        { iDestruct (big_sepL2_nil_inv_r with "Htrtr") as "->". inversion H0. }
+      wp_pures.
+      wp_apply (bhas_length_3_spec with "Hf'") as "_".
+      assert (kF = 2 ∨ kF = 3) as [-> | ->] by invert_all_in; wp_pures.
+      * wp_apply (bis_empty_spec with "Hl") as "_".
+        assert (bool_decide (kL = 0%nat) = false) as -> by invert_all_in.
+        wp_pures.
+        iDestruct (split_time 1 with "τ") as "[ι τ]". by lia.
+        iDestruct (split_time 3 with "τ") as "[ι' τ]". by lia.
+        wp_apply (unsafe_naive_eject with "[ι ι']").
+          { iFrame.
+            iDestruct (strutcure_and_time with "[ι']") as "H".
+              { iFrame.
+                by iExact "Hf". }
+            iExact "H". }
+        iIntros (x' d' o') "(%Hoeq' & Hpush)".
+        wp_pures.
+        apply app_sing_inv in Hoeq' as [-> <-].
+        wp_apply (antinormalize_special_spec with "Ht!") as (t') "Ht''".
+        wp_pures. iModIntro.
+        iApply "Hψ".
+        iFrame.
+        doneL.
+        iLeft.
+        iSplitL "Ht''"; [| iSplitL "τ"].
+        -- iExact "Ht''".
+        -- by iDestruct (split_time (time_for_pop - 4) with "[τ]") as "[ι _]".
+        -- iExact "Hpush".
+      * iDestruct (split_time 1 with "τ") as "[ι τ]". by lia.
+        iDestruct (split_time 3 with "τ") as "[ι' τ]". by lia.
+        wp_apply (unsafe_naive_eject with "[ι ι']").
+          { iFrame.
+            iDestruct (strutcure_and_time with "[ι']") as "H".
+              { iFrame.
+                by iExact "Hf". }
+            iExact "H". }
+        iIntros (x' d' o') "(%Hoeq' & Hpush)".
+        wp_pures.
+        apply app_sing_inv in Hoeq' as [-> <-].
+        wp_apply (antinormalize_special_spec with "Ht!") as (t') "Ht''".
+        wp_pures. iModIntro.
+        iApply "Hψ".
+        iFrame.
+        doneL.
+        iLeft.
+        iSplitL "Ht''"; [| iSplitL "τ"].
+        -- iExact "Ht''".
+        -- by iDestruct (split_time (time_for_pop - 4) with "[τ]") as "[ι _]".
+        -- iExact "Hpush".
+    + wp_pures.
+      rewrite isDeque_unfold.
+      wp_pures.
+      wp_apply (bhas_length_3_spec with "Hf'") as "_".
+      wp_pures.
+      assert (kF = 2 ∨ kF = 3) as [-> | ->] by invert_all_in; wp_pures.
+      * wp_apply (bis_empty_spec with "Hl") as "_".
+        wp_pures.
+        assert (bool_decide (kL = 0%nat) = false) as -> by invert_all_in.
+        wp_pures.
+        iDestruct (split_time 1 with "τ") as "[ι τ]". by lia.
+        iDestruct (split_time 3 with "τ") as "[ι' τ]". by lia.
+        wp_apply (unsafe_naive_eject with "[ι ι']").
+          { iFrame.
+            iDestruct (strutcure_and_time with "[ι']") as "H".
+              { iFrame.
+                by iExact "Hf". }
+            iExact "H". }
+        iIntros (x' d' o') "(%Hoeq' & Hpush)".
+        wp_pures.
+        apply app_sing_inv in Hoeq' as [-> <-].
+        wp_apply (antinormalize_special_spec with "Ht!") as (t') "Ht''".
+        wp_pures. iModIntro.
+        iApply "Hψ".
+        iFrame.
+        doneL.
+        iLeft.
+        iSplitL "Ht''"; [| iSplitL "τ"].
+        -- iExact "Ht''".
+        -- by iDestruct (split_time (time_for_pop - 4) with "[τ]") as "[ι _]".
+        -- iExact "Hpush".
+      * iDestruct (split_time 1 with "τ") as "[ι τ]". by lia.
+        iDestruct (split_time 3 with "τ") as "[ι' τ]". by lia.
+        wp_apply (unsafe_naive_eject with "[ι ι']").
+          { iFrame.
+            iDestruct (strutcure_and_time with "[ι']") as "H".
+              { iFrame.
+                by iExact "Hf". }
+            iExact "H". }
+        iIntros (x' d' o') "(%Hoeq' & Hpush)".
+        wp_pures.
+        apply app_sing_inv in Hoeq' as [-> <-].
+        wp_apply (antinormalize_special_spec with "Ht!") as (t') "Ht''".
+        wp_pures. iModIntro.
+        iApply "Hψ".
+        iFrame.
+        doneL.
+        iLeft.
+        iSplitL "Ht''"; [| iSplitL "τ"].
+        -- iExact "Ht''".
+        -- by iDestruct (split_time (time_for_pop - 4) with "[τ]") as "[ι _]".
+        -- iExact "Hpush".
+    + wp_pures.
+      wp_apply (bhas_length_3_spec with "Hf'") as "_".
+      wp_pures.
+      wp_apply (bis_empty_spec with "Hl") as "_".
+      wp_pures.
+      wp_bind  (eject_nonempty _)%E.
+      iApply (wp_strong_mono with "[iH τ O]").
+        { auto. } { reflexivity. }
+      * iApply ("iH" with "[] [τ]"); [| auto | auto]. iExact "Hd".
+      * iIntros (v) "(%d' & -> & Hd' & O)". iModIntro.
+        wp_pures.
+        wp_apply (antinormalize_not_special_spec with "Ht!") as (t') "Ht''".
+        wp_pures. iModIntro.
+        iApply "Hψ".
+        iFrame. doneL.
+        iRight.
+        iFrame.
+  Unshelve.
+    simpl. apply fiveTuplePersistent.
+  Qed.
+
+  Lemma prepare_eject_spec : forall n o f,
+    {{{ isUnsafeEjectFiveTuple π n o f ∗ ⏱ (time_for_pop - 1) ∗ Token π (S n) ∗
+      ∀ ℓ x o', ℓ ⤇{π , S n} fiveTuple π (S n) (o' ++ ⋅x) -∗
+        ⏱ time_for_pop -∗
+        Token π (S n) -∗
+        WP eject_nonempty #ℓ {{ r, ∃ d, ⌜ r = (d, x)%V ⌝ ∗ isDeque π (S n) o' d ∗ Token π (S n) }}
+    }}}
+      subst "eject_nonempty" eject_nonempty (prepare_eject f)
+    {{{ f' kp ks, RET f'; isEjectFiveTuple n o kp ks f' ∗ Token π (S n) ∗ ⏱ (kp ⊻ ks) }}}.
+  Proof.
+    Opaque eject_triple.
+    iIntros (n o f ψ) "(Hf & τ & O & iH) Hψ".
+    rewrite /isUnsafeEjectFiveTuple.
+    iDestruct "Hf" as "(%p & %l & %m & %r & %s & %op & %ol & %om & %or & %os &
+                      %kPr & %ltr & %rtr &
+                      -> & %conf & pot & #Hp & #Hl & #Hm & #Hr & #Hs &
+                      #Hltr & #Hrtr & %Hoeq)".
+    rewrite /prepare_eject.
+    wp_pures.
+    inversion conf.
+    do 2 rewrite isDeque_unfold.
+    Notation selpat := "[[-> ->] | (%ℓ & -> & Hℓ)]".
+    iDestruct "Hr" as selpat;
+    [iDestruct "Hl" as selpat |].
+    - wp_pures.
+      wp_apply (bhas_length_3_spec with "Hp") as "_".
+      iDestruct (big_sepL2_nil_inv_r with "Hltr") as "->";
+      iDestruct (big_sepL2_nil_inv_r with "Hrtr") as "->".
+      inversion H; wp_pures.
+      + wp_apply (bconcat323_spec with "[Hp Hm Hs]") as "%b' Hb8". by iFrame "#".
+        wp_pures.
+        iApply "Hψ".
+        iModIntro. iSplitR "O τ"; [| iSplitL "O"; [done | ]].
+        * iExists bempty, NONEV, bempty, NONEV, b', [], [], [], [], (op++om++os),
+            0, [], [].
+          iFrame. iFrame "#".
+          doneL.
+          iSplit. by easy_config.
+          iSplit. by (iApply bempty_spec).
+          iSplit. by isEmptyDeque.
+          iSplit. by (iApply bempty_spec).
+          iSplit. by isEmptyDeque.
+          repeat doneL.
+          iPureIntro.
+          aac_rewrite Hoeq.
+          by rewrite //.
+        * simpl. by split_t 3.
+      + assert (bool_decide (kPr = 3%nat) = false) as ->.
+        { clear H H0. invert_all_in. }
+        wp_pures.
+        change (kPr ∈ map S [3;4;5]) in H7.
+        apply decrease_in in H7 as (k & -> & Hk).
+        clear H H0 H6.
+        wp_apply (bdouble_move_right_spec with "[Hp Hm Hs]"). by iFrame "#".
+        iIntros (b1 b2 b3 o1 o2 o3) "(#H1 & #H2 & #H3 & %Heq)".
+        wp_pures.
+        iModIntro.
+        split_ti k 4.
+        iApply "Hψ". iSplitR "O ι"; [| by iFrame].
+        iExists b1, NONEV, b2, NONEV, b3, o1, [], o2, [], o3,
+          2, [], [].
+        iFrame. iFrame "#".
+        doneL.
+        iSplit. iPureIntro. constructor; invert_all_in; list_elem_of.
+        iSplit. by isEmptyDeque.
+        iSplit. by isEmptyDeque.
+        repeat doneL.
+        iPureIntro.
+        aac_rewrite Hoeq.
+        rewrite //.
+    - wp_pures.
+      iDestruct (big_sepL2_nil_inv_r with "Hrtr") as "->".
+      wp_bind (let: "f" := _ in _)%E.
+      iDestruct (time_combine with "[τ pot]") as "τ". by iFrame.
+      iDestruct (split_time time_for_pop with "τ") as "[ι τ']".
+      invert_all_in; simpl; try lia.
+      wp_apply (eject_triple_spec with "[ι O iH]").
+      + iSplit. iExact "Hℓ".
+        iSplitL "O". done.
+        iSplitL "ι". done.
+        iSplit. iExact "Hltr".
+        iApply "iH".
+      + Transparent isSpecialTriple.
+        iIntros (t' t o' rtr' os' d') "(O & [-> ->] & Htr' & [(#Ht & τ & Hd') | (Ht & Hd')])".
+          (* appeler la spec de pop_case_2_special *)
+        * iDestruct "Ht" as (fi c la fc cc lc kF kL tr) "(%tconf & -> & #Hfi & #Hc & #Hla & #Htrtr & %Hleq)".
+          wp_pures.
+          wp_apply (bhas_length_3_spec with "Hla") as "_".
+          inversion tconf; wp_pures.
+          -- wp_apply (bdouble_move_right_spec) as (b1 b2 b3 o1 o2 o3) "(#H1 & #H2 & #H3 & %Hoeq')".
+            { assert (3 = 2 + 1) as -> by reflexivity.
+              iFrame "#". }
+            rewrite /atriple.
+            wp_pures.
+            wp_apply (bis_empty_spec with "Hfi") as "_".
+            inversion H7; rewrite /atriple_.
+            ++ wp_pures.
+              wp_bind (inject _ _)%E.
+              iApply (wp_strong_mono with "Hd'"). { auto. } { auto. }
+              iIntros (l') "Hl'".
+              iModIntro. wp_pures.
+              iModIntro.
+              iApply "Hψ".
+              split_ti kPr 4.
+              iSplitR "O ι"; [| by iFrame].
+              iExists p, l', b2, NONEV, b3,
+                op, (os' ++ ⋅(o1++List.concat cc)), o2, [], o3, 2,
+                (rtr' ++ ⋅(b1, c, bempty)%V), [].
+              doneL.
+              iFrame "#". iFrame.
+              iSplit. iPureIntro. by easy_config.
+              iSplit. by isEmptyDeque.
+              iSplit; [ iApply (big_sepL2_app) |].
+              ** iDestruct (big_sepL2_app_inv with "Hltr") as "[Hrtr' _]". by right.
+                iApply (big_sepL2_mono with "Hrtr'"). by auto.
+              ** simpl; doneR.
+                iNext. iClear "Hrtr".
+                rewrite triple_unfold.
+                iExists b1, c, bempty, o1, cc, [], 2, 0, tr.
+                iSplit. iPureIntro. rewrite -H3. by easy_config.
+                doneL. iFrame "#".
+                iSplit. by iApply bempty_spec.
+                iSplit. iApply (big_sepL2_mono with "Htrtr"). by auto.
+                iPureIntro.
+                rewrite app_nil_r //.
+              ** doneL.
+                iDestruct (buffer_length with "Hfi") as "%Hlfi".
+                destruct fc; [| inversion Hlfi].
+                destruct cc; [| inversion H3].
+                iPureIntro.
+                rewrite Hoeq /= Hleq !concat_app /= app_nil_r.
+                aac_rewrite Hoeq'.
+                aac_reflexivity.
+            ++ assert (bool_decide (kF = 0%nat) = false) as -> by invert_all_in.
+              wp_pures.
+              wp_bind (inject _ _)%E.
+              iApply (wp_strong_mono with "Hd'"). { auto. } { auto. }
+              iIntros (l') "Hl'".
+              iModIntro. wp_pures.
+              iModIntro.
+              iApply "Hψ".
+              split_ti kPr 4.
+              iSplitR "O ι"; [| by iFrame].
+              iExists p, l', b2, NONEV, b3,
+                op, (os' ++ ⋅(fc ++ List.concat cc ++ o1)), o2, [], o3, 2,
+                (rtr' ++ ⋅(fi, c, b1)%V), [].
+              doneL.
+              iFrame "#". iFrame.
+              iSplit. iPureIntro. by easy_config.
+              iSplit. by isEmptyDeque.
+              iSplit; [ iApply (big_sepL2_app) |].
+              ** iDestruct (big_sepL2_app_inv with "Hltr") as "[Hrtr' _]". by right.
+                iApply (big_sepL2_mono with "Hrtr'"). by auto.
+              ** simpl; doneR.
+                iNext. iClear "Hrtr".
+                rewrite triple_unfold.
+                iExists fi, c, b1, fc, cc, o1, kF, 2, tr.
+                iSplit. iPureIntro. rewrite -H3. by easy_config.
+                doneL. iFrame "#".
+                iSplit. iApply (big_sepL2_mono with "Htrtr"). by auto.
+                iPureIntro.
+                rewrite //.
+              ** doneL.
+                iDestruct (buffer_length with "Hfi") as "%Hlfi".
+                destruct cc; [| inversion H3].
+                iPureIntro.
+                rewrite Hoeq /= Hleq !concat_app /= app_nil_r.
+                aac_rewrite Hoeq'.
+                aac_reflexivity.
+          -- assert (kL = 2 ∨ kL = 3) as HkL by (clear H H0 H8; invert_all_in).
+            destruct HkL as [-> | ->]; wp_pures.
+            ++ wp_apply (bconcat23_spec with "[Hm Hs]") as (b') "Hb'". by iFrame "#".
+              wp_pures.
+              rewrite isDeque_unfold.
+              iDestruct "Hc" as "[[_ ->] | (%ℓc & -> & Hℓc)]".
+                { iDestruct (big_sepL2_nil_inv_r with "Htrtr") as "->". inversion H6. }
+              wp_pures.
+              wp_apply (abuffer_spec_explicit with "Hfi") as "Ht". by assumption.
+              wp_pures.
+              wp_bind (inject _ _)%E.
+              iApply (wp_strong_mono with "Hd'"). { auto. } { auto. }
+              iIntros (l') "Hl'".
+              iModIntro. wp_pures.
+              iDestruct (split_time time_for_concat with "τ") as "[ι τ]". by lia.
+              wp_apply (dconcat_spec_helper with "[Hℓc Hl' ι O]") as (l) "[Hl O]".
+                { iFrame. ℓisDeque ℓc. iExact "Hℓc". }
+              wp_pures.
+              iModIntro.
+              iApply "Hψ".
+              split_ti kPr 5.
+              iSplitR "O ι"; [| by iFrame].
+              iExists p, l, la, NONEV, b', op, ((os'++⋅fc)++cc), lc, [], (om++os),
+                2, ((rtr'++⋅(fi, NONEV, bempty)%V)++tr), [].
+              doneL.
+              iSplit. iPureIntro. by easy_config.
+              iFrame. iFrame "#".
+              iSplit. by isEmptyDeque.
+              iSplit.
+              ** iSplit. doneR.
+                iApply (big_sepL2_mono with "Htr'"). by auto.
+                iApply (big_sepL2_mono with "Htrtr"). by auto.
+              ** doneL. iPureIntro.
+                rewrite !concat_app Hoeq Hleq /= !app_nil_r !concat_app /=.
+                aac_reflexivity.
+            ++ wp_apply (bdouble_move_right_spec with "[Hla Hm Hs]").
+                { iFrame "#". assert (3 = 2 + 1) as -> by reflexivity. done. }
+             iIntros (b1 b2 b3 o1 o2 o3) "(H1 & H2 & #H3 & %Hnoeq)".
+              rewrite /atriple.
+              wp_pures.
+              wp_apply (bis_empty_spec with "Hfi") as "_".
+              assert (bool_decide (kF = 0%nat) = false) as -> by invert_all_in.
+              rewrite /atriple_.
+              wp_pures.
+              wp_bind (inject _ _)%E.
+              iApply (wp_strong_mono with "Hd'"). { auto. } { auto. }
+              iIntros (l') "Hl'".
+              iModIntro.
+              wp_pures.
+              iModIntro. iApply "Hψ".
+              split_ti kPr 4.
+              iSplitR "O ι"; [| by iFrame].
+              iExists p, l', b2, NONEV, b3,
+                op, (os'++⋅(fc++List.concat cc++o1)), o2, [], o3,
+                2, (rtr'++⋅(fi, c, b1)%V), [].
+              doneL.
+              iSplit. iPureIntro. simpl. by easy_config.
+              iFrame "#". iFrame.
+              iSplit. by isEmptyDeque.
+              iSplit; [ iApply (big_sepL2_app with "[Htr']") | doneL ].
+              ** iApply (big_sepL2_mono with "Htr'"). by auto.
+              ** simpl. doneR. iNext.
+                rewrite !triple_unfold.
+                iExists fi, c, b1, fc, cc, o1, kF, 2, tr.
+                iSplit. iPureIntro. by easy_config.
+                doneL.
+                iFrame . iFrame "#".
+                iSplit. iApply (big_sepL2_mono with "Htrtr"). by auto.
+                done.
+              ** iPureIntro.
+                rewrite !concat_app Hoeq Hleq /= !app_nil_r concat_app /=.
+                aac_rewrite Hnoeq.
+                aac_reflexivity.
+          -- assert (kL = 2 ∨ kL = 3) as HkL by (clear H H0 H8; invert_all_in).
+            destruct HkL as [-> | ->]; wp_pures.
+            ++ wp_apply (bconcat23_spec with "[Hm Hs]") as (b') "Hb'". by iFrame "#".
+              wp_pures.
+              destruct (bool_decide (c = NONEV)); wp_pures.
+              ** wp_apply (bis_empty_spec with "Hfi") as "_".
+                assert (bool_decide (kF = 0%nat) = false) as -> by invert_all_in.
+                wp_pures.
+                wp_apply (abuffer_spec_explicit with "Hfi") as "Ht". by assumption.
+                wp_pures.
+                wp_bind (inject _ _)%E.
+                iApply (wp_strong_mono with "Hd'"). { auto. } { auto. }
+                iIntros (l') "Hl'".
+                iModIntro. wp_pures.
+                iDestruct (split_time time_for_concat with "τ") as "[ι τ]". by lia.
+                wp_apply (dconcat_spec_helper with "[Hc Hl' ι O]") as (l) "[Hl O]".
+                  { iFrame. by iFrame "#". }
+                wp_pures.
+                iModIntro.
+                iApply "Hψ".
+                split_ti kPr 5.
+                iSplitR "O ι"; [| by iFrame].
+                iExists p, l, la, NONEV, b', op, ((os'++⋅fc)++cc), lc, [], (om++os),
+                2, ((rtr'++⋅(fi, NONEV, bempty)%V)++tr), [].
+                doneL.
+                iSplit. iPureIntro. by easy_config.
+                iFrame. iFrame "#".
+                iSplit. by isEmptyDeque.
+                iSplit.
+                --- iSplit. doneR.
+                  iApply (big_sepL2_mono with "Htr'"). by auto.
+                  iApply (big_sepL2_mono with "Htrtr"). by auto.
+                --- doneL. iPureIntro.
+                  rewrite !concat_app Hoeq Hleq /= !app_nil_r !concat_app /=.
+                  aac_reflexivity.
+              ** wp_apply (abuffer_spec_explicit with "Hfi") as "Ht". by assumption.
+                wp_pures.
+                wp_bind (inject _ _)%E.
+                iApply (wp_strong_mono with "Hd'"). { auto. } { auto. }
+                iIntros (l') "Hl'".
+                iModIntro. wp_pures.
+                iDestruct (split_time time_for_concat with "τ") as "[ι τ]". by lia.
+                wp_apply (dconcat_spec_helper with "[Hc Hl' ι O]") as (l) "[Hl O]".
+                  { iFrame. by iFrame "#". }
+                wp_pures.
+                iModIntro.
+                iApply "Hψ".
+                split_ti kPr 5.
+                iSplitR "O ι"; [| by iFrame].
+                iExists p, l, la, NONEV, b', op, ((os'++⋅_)++cc), lc, [], (om++os),
+                  2, ((rtr'++⋅(fi, NONEV, bempty)%V)++tr), [].
+                doneL.
+                iSplit. iPureIntro. by easy_config.
+                iFrame. iFrame "#".
+                iSplit. by isEmptyDeque.
+                iSplit; [| doneL].
+                --- iSplit. doneR.
+                  iApply (big_sepL2_mono with "Htr'"). by auto.
+                  iApply (big_sepL2_mono with "Htrtr"). by auto.
+                --- iPureIntro.
+                  rewrite !concat_app Hoeq Hleq /= !app_nil_r concat_app /=.
+                  aac_reflexivity.
+            ++ wp_apply (bdouble_move_right_spec) as (b1 b2 b3 o1 o2 o3) "(#H1 & #H2 & #H3 & %Hoeq')".
+            { assert (3 = 2 + 1) as -> by reflexivity.
+              iFrame "#". }
+            rewrite /atriple.
+            wp_pures.
+            wp_apply (bis_empty_spec with "Hfi") as "_".
+            assert (bool_decide (kF = 0%nat) = false) as -> by invert_all_in.
+            rewrite /atriple_.
+            wp_pures.
+            wp_bind (inject _ _)%E.
+            iApply (wp_strong_mono with "Hd'"). { auto. } { auto. }
+            iIntros (l') "Hl'".
+            iModIntro. wp_pures.
+            iModIntro.
+            iApply "Hψ".
+            split_ti kPr 4.
+            iSplitR "O ι"; [| by iFrame].
+            iExists p, l', b2, NONEV, b3,
+                op, (os'++⋅(fc++List.concat cc++o1)), o2, [], o3,
+                2, (rtr'++⋅(fi, c, b1)%V), [].
+            doneL.
+            iSplit. iPureIntro. simpl. by easy_config.
+            iFrame "#". iFrame.
+            iSplit. by isEmptyDeque.
+            iSplit; [ iApply (big_sepL2_app with "[Htr']") | doneL ].
+            ** iApply (big_sepL2_mono with "Htr'"). by auto.
+            ** simpl. doneR. iNext.
+              rewrite !triple_unfold.
+              iExists fi, c, b1, fc, cc, o1, kF, 2, tr.
+              iSplit. iPureIntro. destruct (length cc); constructor; (list_elem_of || lia).
+              doneL.
+              iFrame . iFrame "#".
+              iSplit. iApply (big_sepL2_mono with "Htrtr"). by auto.
+              done.
+            ** iPureIntro.
+              rewrite !concat_app Hoeq Hleq /= !app_nil_r concat_app /=.
+              aac_rewrite Hoeq'.
+              aac_reflexivity.
+        Opaque isSpecialTriple.
+        * Transparent isNotSpecialTriple. wp_pures.
+          (* appeler la spec de pop_case_2_not_special *)
+          rewrite /prepare_pop_case_2.
+          iDestruct "τ'" as "τ".
+          iDestruct "Ht" as (fi c la fc cc lc kF kL tr) "(%tconf & -> & #Hfi & #Hc & #Hla & #Htrtr & %Hleq)".
+          wp_pures.
+          wp_apply (bhas_length_3_spec with "Hla") as "_".
+          inversion tconf; wp_pures.
+          wp_apply (bconcat23_spec with "[Hm Hs]") as (b') "Hb'". by iFrame "#".
+          rewrite isDeque_unfold.
+          iDestruct "Hc" as "[[-> ->] | (%ℓ' & -> & Hℓ')]".
+          2: {
+            iDestruct (na_own_acc (↑ W (S n)) with "O") as "[O A]". by apply access_stage.
+            iInv "Hℓ'" as "[(%v' & Hv' & Hℓ'') O]".
+            wp_pure.
+            iExFalso.
+            iDestruct "Hv'" as (pr' ld' md' rd' sf' pc' lc' mc' rc' sc' kp' km' ks' lt rt) "(_ & %conf' & _ & _ & _ & _ & _ & Hs' & _ & _ & ->)".
+            iDestruct (big_sepL2_length with "Htrtr") as "%Hlen".
+            rewrite Hlen in H7.
+            iDestruct (buffer_length with "Hs'") as "%Hslen".
+            assert (ks' > 0) as Hslen' by (inversion conf'; invert_all_in; lia).
+            rewrite !length_app in H7.
+            lia.
+          }
+          wp_pures.
+          wp_apply (bis_empty_spec with "Hfi") as "_".
+          wp_pures.
+          (*
+          assert (kL = 0 ∨ kL ∈ [2; 3]) as Hkl. by invert_all_in.
+          destruct Hkl as [-> | Hkl]; wp_pures.
+          -- *)
+            iModIntro. iApply "Hψ".
+            split_ti kPr 5.
+            iSplitR "O ι"; [| by iFrame].
+            iExists p, d', la, NONEV, b', op, os', lc, [], (om++os),
+              2, rtr', [].
+            doneL.
+            iSplit. iPureIntro. by easy_config.
+            iFrame "#". iFrame.
+            iSplit. by isEmptyDeque.
+            iSplit. iApply (big_sepL2_mono with "Htr'"). by auto.
+            doneL.
+            destruct fc; [| iDestruct (buffer_length with "Hfi") as "%No"; by inversion No ].
+            destruct cc; [| by inversion H6 ].
+            iPureIntro.
+            rewrite Hoeq Hleq /= concat_app /=.
+            aac_reflexivity.
+        Opaque isNotSpecialTriple.
+    - wp_pures.
+      wp_bind (let: "f" := _ in _)%E.
+      iDestruct (time_combine with "[τ pot]") as "τ". by iFrame.
+      iDestruct (split_time time_for_pop with "τ") as "[ι τ']".
+      invert_all_in; simpl; lia.
+      wp_apply (eject_triple_spec with "[ι O iH]").
+      + iSplit. iExact "Hℓ".
+        iSplitL "O". done.
+        iSplitL "ι". done.
+        iSplit. iExact "Hrtr".
+        iApply "iH".
+      + Transparent isSpecialTriple.
+        iIntros (t' t o' rtr' os' d') "(O & [-> ->] & Htr' & [(#Ht & τ & Hd') | (Ht & Hd')])".
+        * (* appeler la spec de pop_case_1_special *)
+          iDestruct "Ht" as (fi c la fc cc lc kF kL tr) "(%tconf & -> & #Hfi & #Hc & #Hla & #Htrtr & %Hleq)".
+          wp_pures.
+          wp_apply (bhas_length_3_spec with "Hla") as "_".
+          inversion tconf; wp_pures.
+          -- wp_apply (bmove_right_1_33_spec with "[Hla Hs]"). by iFrame "#".
+            iIntros (b1 b2 o1 o2) "(#H1 & #H2 & %Honeq)".
+            rewrite /atriple.
+            wp_pures.
+            wp_apply (bis_empty_spec with "Hfi") as "_".
+            inversion H7; rewrite /atriple_.
+            ++ wp_pures.
+              wp_bind (inject _ _)%E.
+              iApply (wp_strong_mono with "Hd'"). { auto. } { auto. }
+              iIntros (r') "Hr'".
+              iModIntro. wp_pures.
+              iModIntro. iApply "Hψ".
+              split_ti kPr 4.
+              iSplitR "O ι"; [| by iFrame].
+              iExists p, l, m, r', b2, op, ol, om, (os'++⋅(fc++List.concat cc++o1)), o2,
+                2, ltr, (rtr' ++ ⋅(b1, c, bempty)%V).
+              doneL.
+              iSplit. iPureIntro. by easy_config.
+              rewrite -isDeque_unfold.
+              iFrame. iFrame "#".
+              iSplit. iApply (big_sepL2_mono with "Hltr"). by auto.
+              iSplit. iApply (big_sepL2_app with "[Htr']"). iApply (big_sepL2_mono with "Htr'"). by auto.
+              simpl. doneR. iNext.
+                iClear "Hltr".
+                rewrite triple_unfold.
+                iExists b1, c, bempty, o1, cc, [], 2, 0, tr.
+                iSplit. iPureIntro. inversion H3. by easy_config.
+                doneL.
+                iFrame "#".
+                iSplit. by iApply bempty_spec.
+                iSplit. iApply (big_sepL2_mono with "Htrtr"). by auto.
+                destruct fc; [| iDestruct (buffer_length with "Hfi") as "%No"; by inversion No ].
+                destruct cc; [| by inversion H6 ].
+                iPureIntro. rewrite /= app_nil_r //.
+              iPureIntro.
+                rewrite Hoeq /= Hleq !concat_app /=.
+                aac_rewrite Honeq.
+                aac_reflexivity.
+            ++ assert (bool_decide (kF = 0%nat) = false) as -> by invert_all_in.
+              wp_pures.
+              wp_bind (inject _ _)%E.
+              iApply (wp_strong_mono with "Hd'"). { auto. } { auto. }
+              iIntros (r') "Hr'".
+              iModIntro. wp_pures.
+              iModIntro. iApply "Hψ".
+              split_ti kPr 4.
+              iSplitR "O ι"; [| by iFrame].
+              iExists p, l, m, r', b2, op, ol, om, (os'++⋅(fc++List.concat cc++o1)), o2,
+                2, ltr, (rtr' ++ ⋅(fi, c, b1)%V).
+              doneL.
+              iSplit. iPureIntro. by easy_config.
+              rewrite -isDeque_unfold.
+              iFrame. iFrame "#".
+              iSplit. iApply (big_sepL2_mono with "Hltr"). by auto.
+              iSplit. iApply (big_sepL2_app with "[Htr']"). iApply (big_sepL2_mono with "Htr'"). by auto.
+              simpl. doneR. iNext.
+                iClear "Hltr".
+                rewrite triple_unfold.
+                iExists fi, c, b1, fc, cc, o1, kF, 2, tr.
+                iSplit. iPureIntro. inversion H3. by easy_config.
+                doneL.
+                iFrame "#".
+                iSplit. iApply (big_sepL2_mono with "Htrtr"). by auto.
+                destruct fc; [| iDestruct (buffer_length with "Hfi") as "%No"; by inversion No ].
+                destruct cc; [| by inversion H6 ].
+                iPureIntro. rewrite //.
+              iPureIntro.
+                rewrite Hoeq /= Hleq !concat_app /=.
+                aac_rewrite Honeq.
+                aac_reflexivity.
+          -- assert (kL = 2 ∨ kL = 3) as [-> | ->] by invert_all_in; wp_pures.
+            ++ wp_apply (bconcat23_spec with "[Hla Hs]") as (b') "Hb'". by iFrame "#".
+              wp_pures.
+              rewrite !isDeque_unfold.
+              iDestruct "Hc" as "[[-> ->] | (%ℓc & -> & Hℓc)]".
+                { iDestruct (big_sepL2_nil_inv_r with "Htrtr") as "->". inversion H6. }
+              wp_pures.
+              wp_apply (abuffer_spec_explicit with "Hfi") as "Ht". by assumption.
+              wp_pures.
+              wp_bind (inject _ _)%E.
+              iApply (wp_strong_mono with "Hd'"). { auto. } { auto. }
+              iIntros (r') "Hr'".
+              iModIntro. wp_pures.
+              iDestruct (split_time time_for_concat with "τ") as "[ι τ]". by lia.
+              wp_apply (dconcat_spec_helper with "[Hℓc Hr' ι O]") as (r) "[Hr O]".
+                { iFrame. ℓisDeque ℓc. iExact "Hℓc". }
+              wp_pures.
+              iModIntro.
+              iApply "Hψ".
+              split_ti kPr 5.
+              iSplitR "O ι"; [| by iFrame].
+              iExists p, l, m, r, b', op, ol, om, ((os' ++ ⋅fc) ++ cc), (lc ++ os),
+                2, ltr, ((rtr'++⋅(fi, NONEV, bempty)%V)++tr).
+              doneL.
+              iSplit. iPureIntro. simpl. by easy_config.
+              rewrite -isDeque_unfold.
+              iFrame "#". iFrame.
+              iSplit; [| iSplit; [iSplit; [iSplit; [| done] |] |]].
+              ** iApply (big_sepL2_mono with "Hltr"). by auto.
+              ** iApply (big_sepL2_mono with "Htr'"). by auto.
+              ** iApply (big_sepL2_mono with "Htrtr"). by auto.
+              ** iPureIntro.
+                rewrite Hoeq Hleq !concat_app /=.
+                aac_reflexivity.
+            ++ wp_apply (bmove_right_1_33_spec with "[Hla Hs]"). by iFrame "#".
+              iIntros (b1 b2 o1 o2) "(#H1 & #H2 & %Hnoeq)".
+              rewrite /atriple.
+              wp_pures.
+              wp_apply (bis_empty_spec with "Hfi") as "_".
+              assert (bool_decide (kF = 0%nat) = false) as -> by invert_all_in.
+              rewrite /atriple_.
+              wp_pures.
+              wp_bind (inject _ _)%E.
+              iApply (wp_strong_mono with "Hd'"). { auto. } { auto. }
+              iIntros (r') "Hr'".
+              iModIntro. wp_pures.
+              iApply "Hψ".
+              split_ti kPr 4.
+              iSplitR "O ι"; [| by iFrame].
+              iModIntro.
+              iExists p, l, m, r', b2, op, ol, om, (os'++⋅(fc++List.concat cc++o1)), o2,
+                2, ltr, (rtr'++⋅(fi, c, b1)%V).
+              doneL.
+              iSplit. iPureIntro. simpl. by easy_config.
+              rewrite -isDeque_unfold.
+              iFrame "#". iFrame.
+              iSplit. iApply (big_sepL2_mono with "Hltr"). by auto.
+              iSplit. iApply (big_sepL2_app with "[Htr']"). iApply (big_sepL2_mono with "Htr'"). by auto.
+              iSplit.
+                iClear "Hltr".
+                rewrite triple_unfold.
+                iExists fi, c, b1, fc, cc, o1, kF, 2, tr.
+                iSplitL. iPureIntro. destruct (length cc); [inversion H6 |]; by easy_config.
+                doneL.
+                iFrame "#".
+                iSplit. iApply (big_sepL2_mono with "Htrtr"). by auto.
+                done.
+              done.
+              iPureIntro.
+                rewrite Hoeq Hleq !concat_app /=.
+                aac_rewrite Hnoeq.
+                aac_reflexivity.
+          -- assert (kL = 2 ∨ kL = 3) as [-> | ->] by invert_all_in; wp_pures.
+            ++ wp_apply (bconcat23_spec with "[Hla Hs]") as (b') "Hb'". by iFrame "#".
+              wp_pures.
+              wp_bind (if: _ then _ else #false)%E.
+              iApply (wp_strong_mono _ _ _ _ _ (λ v, ⌜ v = #false ⌝)%I). { auto. } { auto. }
+                { destruct (bool_decide (c = NONEV)); wp_pures.
+                - wp_apply (bis_empty_spec with "Hfi") as "_".
+                  assert (bool_decide (kF = 0%nat) = false) as -> by invert_all_in.
+                  done.
+                - done.
+                }
+              iIntros (v) "->". iModIntro. wp_pures.
+              wp_apply (abuffer_spec_explicit with "Hfi") as "Ht". by assumption.
+              wp_pures.
+              wp_bind (inject _ _)%E.
+              iApply (wp_strong_mono with "Hd'"). { auto. } { auto. }
+              iIntros (r') "Hr'".
+              iModIntro. wp_pures.
+              iDestruct (split_time time_for_concat with "τ") as "[ι τ]". by lia.
+              wp_apply (dconcat_spec_helper with "[Hc Hr' ι O]") as (r) "[Hr O]".
+                { iFrame. iExact "Hc". }
+              wp_pures.
+              iModIntro.
+              iApply "Hψ".
+              split_ti kPr 5.
+              iSplitR "O ι"; [| by iFrame].
+              iExists p, l, m, r, b', op, ol, om, ((os' ++ ⋅fc) ++ cc), (lc ++ os),
+                2, ltr, ((rtr'++⋅(fi, NONEV, bempty)%V)++tr).
+              doneL.
+              iSplit. iPureIntro. simpl. by easy_config.
+              rewrite -isDeque_unfold.
+              iFrame "#". iFrame.
+              iSplit; [| iSplit; [iSplit; [iSplit; [| done] |] |]].
+              ** iApply (big_sepL2_mono with "Hltr"). by auto.
+              ** iApply (big_sepL2_mono with "Htr'"). by auto.
+              ** iApply (big_sepL2_mono with "Htrtr"). by auto.
+              ** iPureIntro.
+                rewrite Hoeq Hleq !concat_app /=.
+                aac_reflexivity.
+            ++ wp_apply (bmove_right_1_33_spec with "[Hla Hs]"). by iFrame "#".
+              iIntros (b1 b2 o1 o2) "(#H1 & #H2 & %Hnoeq)".
+              rewrite /atriple.
+              wp_pures.
+              wp_apply (bis_empty_spec with "Hfi") as "_".
+              assert (bool_decide (kF = 0%nat) = false) as -> by invert_all_in.
+              rewrite /atriple_.
+              wp_pures.
+              wp_bind (inject _ _)%E.
+              iApply (wp_strong_mono with "Hd'"). { auto. } { auto. }
+              iIntros (r') "Hr'".
+              iModIntro. wp_pures.
+              iApply "Hψ".
+              split_ti kPr 4.
+              iSplitR "O ι"; [| by iFrame].
+              iModIntro.
+              iExists p, l, m, r', b2, op, ol, om, (os'++⋅(fc++List.concat cc++o1)), o2,
+                2, ltr, (rtr' ++ ⋅(fi, c, b1)%V).
+              doneL.
+              iSplit. iPureIntro. by easy_config.
+              rewrite -isDeque_unfold.
+              iFrame. iFrame "#".
+              iSplit. iApply (big_sepL2_mono with "Hltr"). by auto.
+              iSplit. iApply (big_sepL2_app with "[Htr']"). iApply (big_sepL2_mono with "Htr'"). by auto.
+              simpl. doneR. iNext.
+                iClear "Hltr".
+                rewrite triple_unfold.
+                iExists fi, c, b1, fc, cc, o1, kF, 2, tr.
+                iSplit. iPureIntro. destruct (length cc); constructor; by (lia || list_elem_of).
+                doneL.
+                iFrame "#".
+                iSplit. iApply (big_sepL2_mono with "Htrtr"). by auto.
+                destruct fc; [| iDestruct (buffer_length with "Hfi") as "%No"; by inversion No ].
+                destruct cc; [| by inversion H6 ].
+                iPureIntro. rewrite //.
+              iPureIntro.
+                rewrite Hoeq /= Hleq !concat_app /=.
+                aac_rewrite Hnoeq.
+                aac_reflexivity.
+        Opaque isSpecialTriple.
+        * Transparent isNotSpecialTriple.
+          (* appeler la spec de pop_case_1_not_special *)
+          iDestruct "Ht" as (fi c la fc cc lc kF kL tr) "(%tconf & -> & #Hfi & #Hc & #Hla & #Htrtr & %Hleq)".
+          wp_pures.
+          wp_apply (bhas_length_3_spec with "Hla") as "_".
+          inversion tconf; wp_pures.
+          wp_apply (bconcat23_spec with "[Hm Hs]") as (b') "Hb'". by iFrame "#".
+          wp_pures.
+          rewrite !isDeque_unfold.
+          iDestruct "Hc" as "[[-> ->] | (%ℓ' & -> & Hℓ')]".
+          2: {
+            iDestruct (na_own_acc (↑ W (S n)) with "O") as "[O A]". by apply access_stage.
+            iInv "Hℓ'" as "[(%v' & Hv' & Hℓ'') O]".
+            wp_pure.
+            iExFalso.
+            iDestruct "Hv'" as (pr' ld' md' rd' sf' pc' lc' mc' rc' sc' kp' km' ks' lt rt) "(_ & %conf' & _ & _ & _ & _ & _ & Hs' & _ & _ & ->)".
+            iDestruct (big_sepL2_length with "Htrtr") as "%Hlen".
+            rewrite Hlen in H7.
+            iDestruct (buffer_length with "Hs'") as "%Hslen".
+            assert (ks' > 0) as Hslen' by (inversion conf'; invert_all_in; lia).
+            rewrite !length_app in H7.
+            lia.
+          }
+          wp_pures.
+          wp_apply (bis_empty_spec with "Hfi") as "_".
+          wp_pures.
+          iModIntro. iApply "Hψ".
+          iDestruct "τ'" as "τ".
+          split_ti kPr 5.
+          iSplitR "O ι"; [| by iFrame].
+          iExists p, l, m, d', b', op, ol, om, os', (lc++os),
+            2, ltr, rtr'.
+          rewrite -!isDeque_unfold.
+          doneL.
+          iSplit. iPureIntro. by easy_config.
+          iFrame "#". iFrame.
+          iSplit. iApply (big_sepL2_mono with "Hltr"). by auto.
+          iSplit. iApply (big_sepL2_mono with "Htr'"). by auto.
+          destruct fc; [| iDestruct (buffer_length with "Hfi") as "%No"; by inversion No ].
+          destruct cc; [| by inversion H6 ].
+          iPureIntro.
+          rewrite Hoeq Hleq /= concat_app /=.
+          aac_reflexivity.
+        Opaque isNotSpecialTriple.
+    Qed.
+
+  Global Instance isPopFiveTuplePersistent n o kp ks d : Persistent (isEjectFiveTuple n o kp ks d).
+  Proof.
+    rewrite /isEjectFiveTuple.
+    repeat (apply bi.exist_persistent; intro).
+    repeat (apply bi.sep_persistent; apply _).
+  Qed.
+
+End lemmas.
+
+Notation "kp ∘ ks" := (kp ⋄ ks - 1).
+Notation "kp ⊻ ks" := ((kp ∘ ks) + (kp ⋄ ks)) (at level 60).
+
+Ltac split_t τ := iDestruct (split_time τ with "τ") as "[ι τ]"; [ try lia |].
+Ltac split_ti kp ks := iDestruct (split_time (kp ⊻ ks) with "τ") as "[ι τ]"; [ invert_all_in; simpl; try lia |].
+Ltac split_Δ kp ks := split_t (Z.to_nat (Δ kp ks)); [ try (invert_all_in; rewrite /Δ /=; lia) |].
+Ltac gather_t pot := iDestruct (time_combine with String.concat "" ["[τ "; pot; "]"]) as "τ"; [ iFrame |].
