theories/push_corr.v
@@ -1,0 +1,285 @@
+From iris.heap_lang Require Import lang proofmode notation.
+From iris.bi Require Import derived_laws.
+
+From Coq Require Import List.
+Import ListNotations.
+
+From AAC_tactics Require Import AAC.
+From AAC_tactics Require Import Instances.
+Import Instances.Lists.
+
+From Deque Require Import common tick shared_ref deque_corr.
+
+Section proof.
+
+  Context `{!heapGS Σ}.
+
+  (* since this is a functional correction proof, we use a cheat that is confined to this section *)
+  Let TIME_CHEAT : ∀ k, ⊢ (⏱ k : iProp Σ).
+  Admitted.
+
+  Lemma push_spec_helper oD x d :
+    {{{ isDeque oD d }}}
+      push x d
+    {{{ d', RET d'; isDeque (⋅x ++ oD) d' }}}.
+  Proof.
+    iLöb as "iH" forall (x d oD).
+    iIntros (ψ) "Hd Hψ".
+    rewrite /push.
+    iDestruct (TIME_CHEAT 1) as "ι".
+    wp_pures.
+    wp_apply (tick_spec with "ι") as "_".
+    wp_pures.
+    rewrite {1} isDeque_unfold.
+    iDestruct "Hd" as "[[-> ->] | (%ℓ & -> & #Hℓ)]".
+    - wp_pures.
+      rewrite /asingleton. wp_pures.
+      wp_apply bpush_spec as "%b #Hb".
+        { iApply bempty_spec. }
+      wp_pures.
+      wp_bind (ref _)%E.
+      wp_apply (csref_alloc (fiveTuple (⋅x))) as "%ℓ #Hℓ".
+      + rewrite app_nil_r. by iApply (singleton_deque_better).
+      + wp_pures.
+        iApply "Hψ".
+        iFrame.
+        ℓisDeque ℓ. iModIntro. rewrite !app_nil_r //.
+    - wp_pures.
+      wp_apply (csref_load (fiveTuple _)) as "%d #πd".
+        { iFrame. iExact "Hℓ". }
+      iCombine "πd πd" as "[_ Hv]".
+      iDestruct "πd" as "
+        (%pr & %ld & %md & %rd & %sf & %prC & %ldC & %mdC & %rdC & %sfC
+            & %kPr & %kMd & %kSf & %ltr & %rtr & -> & %cfg
+            & #Hpr & #Hld & #Hmd & #Hrd & #Hsf & #Hltr & #Hrtr & %Heq)".
+      wp_pures.
+      wp_bind (if: _ then _ else _)%E.
+      wp_apply (bis_empty_spec with "Hmd") as "_".
+      wp_pures.
+      destruct (bool_decide (kMd = 0)) eqn:?.
+      + apply bool_decide_eq_true_1 in Heqb as Heqmd.
+        wp_pures.
+        wp_bind (if: _ then _ else _)%E.
+        wp_apply (bhas_length_8_spec with "Hsf") as "_".
+        wp_pures.
+        destruct (bool_decide (kSf = 8)) eqn:?.
+        * apply bool_decide_eq_true_1 in Heqb0 as ->.
+          inversion cfg; invert_all_in; destruct ldC; inversion H; destruct rdC; inversion H1.
+          iDestruct (big_sepL2_nil_inv_l with "Hltr") as "->".
+          iDestruct (big_sepL2_nil_inv_l with "Hrtr") as "->".
+          iDestruct (buffer_length with "Hpr") as "%HlprC". destruct prC; [| inversion HlprC].
+          iDestruct (buffer_length with "Hmd") as "%HlmdC". destruct mdC; [| inversion HlmdC].
+          wp_pures.
+          wp_apply (bsplit8_spec with "Hsf") as "%b1 %b2 %b3 %o1 %o2 %o3 (#Hb1 & #Hb2 & #Hb3 & %H123)".
+          wp_pures.
+          wp_bind (#ℓ <- _)%E.
+          wp_apply (csref_store).
+          {
+            iSplit. iExact "Hℓ".
+            iExists b1, ld, b2, rd, b3,
+              o1, [], o2, [], o3,
+              3, 2, 3, [], [].
+            iFrame. iFrame "#".
+            doneL.
+            iSplitR. by easy_config.
+            do 2 doneL.
+            inversion cfg; [| exfalso; lia].
+            iPureIntro.
+            rewrite Heq //=.
+          }
+          iIntros (unit).
+          wp_pures; clear unit.
+          wp_bind (bpush _ _)%E.
+          wp_apply (bpush_spec with "Hb1") as "%pr'' #Hpr''".
+          rewrite /assemble_.
+          wp_pures.
+          wp_bind (ref _)%E.
+          wp_apply (csref_alloc (fiveTuple (⋅x ++ oD))) as "%ℓ' #Hℓ'".
+          -- iExists pr'', ld, b2, rd, b3,
+              (⋅x ++ o1), [], o2, [], o3,
+              4, 2, 3, [], [].
+            iFrame. iFrame "#".
+            doneL.
+            iSplitR. by easy_config.
+            do 2 doneL.
+            inversion cfg; [| exfalso; lia].
+            iPureIntro.
+            rewrite Heq H123 //=.
+          -- wp_pures.
+            iApply "Hψ".
+            iFrame.
+            ℓisDeque ℓ'.
+            iExact "Hℓ'".
+        * wp_pures.
+          apply bool_decide_eq_false_1 in Heqb0.
+          wp_bind (#ℓ <- _)%E.
+          wp_apply (csref_store).
+          {
+            iSplit. iExact "Hℓ".
+            iFrame.
+            iApply (laterInFiveTuple with "Hv").
+          }
+          iIntros (unit).
+          wp_pures; clear unit.
+          rewrite /assemble_.
+          wp_apply (bpush_spec with "Hsf") as "%sf' #Hsf'".
+          wp_pures.
+          wp_apply (csref_alloc (fiveTuple (⋅x ++ oD))) as "%ℓ' #Hℓ'".
+          -- iExists bempty, empty, bempty, empty, sf',
+              [], [], [], [], (⋅x ++ sfC),
+              0, 0, (S kSf), [], [].
+            inversion cfg; [| exfalso; lia ].
+            iDestruct (buffer_length with "Hpr") as "%HlprC". destruct prC; [| inversion HlprC].
+            iDestruct (buffer_length with "Hmd") as "%HlmdC". destruct mdC; [| inversion HlmdC].
+            symmetry in H; rewrite (nil_length_inv _ H) in Heq |- *.
+            symmetry in H1; rewrite (nil_length_inv _ H1) in Heq |- *.
+            iDestruct (big_sepL2_nil_inv_l with "Hltr") as "->".
+            iDestruct (big_sepL2_nil_inv_l with "Hrtr") as "->".
+            iFrame.
+            doneL.
+            iSplitR; [ iPureIntro; constructor; invert_all_in; list_elem_of |].
+            iSplitR. by iApply bempty_spec.
+            iSplitR. by isEmptyDeque.
+            iSplitR. by iApply bempty_spec.
+            iSplitR. by isEmptyDeque.
+            assert (S kSf = kSf + 1) as -> by lia.
+            doneL.
+            aac_normalise in Heq.
+            rewrite Heq.
+            repeat doneL.
+            iPureIntro; simpl; aac_reflexivity.
+          -- wp_pures.
+            iApply "Hψ".
+            iFrame.
+            ℓisDeque ℓ'.
+            iExact "Hℓ'".
+      + apply bool_decide_eq_false_1 in Heqb as Heqmd.
+        wp_pures.
+        wp_apply (bhas_length_6_spec with "Hpr") as "_".
+        wp_pures.
+        destruct (bool_decide (kPr = 6)) eqn:?.
+        * apply bool_decide_eq_true_1 in Heqb0 as ->.
+          wp_pures.
+          wp_apply (bsplit642_spec with "Hpr") as "%b1 %b2 %o1 %o2 (#Ho1 & #Ho2 & %Heq12)".
+          rewrite /abuffer /atriple_.
+          iSpecialize ("iH" $! (b2, NONEV, bempty)%V ld ltr).
+          do 16 wp_pure.
+          wp_smart_apply ("iH") as "%ld' #Hld'"; iClear "iH".
+            by iFrame "#".
+          wp_pures.
+          wp_bind (#ℓ <- _)%E.
+          inversion cfg.
+          wp_apply csref_store.
+          {
+            iSplit. iExact "Hℓ".
+            iExists b1, ld', md, rd, sf,
+              o1, (⋅o2 ++ ldC), mdC, rdC, sfC,
+              4, 2, kSf, (⋅(b2, NONEV, bempty)%V ++ ltr), rtr.
+            iFrame "#".
+            iSplitR. done.
+            iSplitR. { iPureIntro; constructor; list_elem_of. }
+            iSplitL.
+              { iApply (big_sepL2_app with "[Hltr]").
+                - iApply (big_sepL2_singleton).
+                  iNext. rewrite triple_unfold.
+                  iExists b2, NONEV, bempty,
+                    o2, [], [],
+                    2, 0, [].
+                  iSplitR. { iPureIntro; eapply left_leaning; list_elem_of.  }
+                  do 2 doneL.
+                  iSplitR. isEmptyDeque.
+                  iSplitR. iApply bempty_spec.
+                  doneL.
+                  iPureIntro; simpl; aac_reflexivity.
+                - iApply (big_sepL2_mono with "Hltr").
+                  by auto.
+              }
+            iSplitR. iApply (big_sepL2_mono with "Hrtr"). by auto.
+            iPureIntro.
+            rewrite Heq Heq12 /=.
+            aac_reflexivity.
+          }
+          iIntros (unit).
+          rewrite /assemble_.
+          wp_pures; clear unit.
+          wp_apply (bpush_spec with "Ho1") as "%pr3 #Hpr3".
+          wp_pures.
+          wp_apply (csref_alloc (fiveTuple (⋅x ++ oD))) as "%ℓ' #Hℓ'". {
+            iExists pr3, ld', md, rd, sf,
+              (⋅x ++ o1), (⋅o2 ++ ldC), mdC, rdC, sfC,
+              5, 2, kSf, (⋅ (b2, NONEV, bempty)%V ++ ltr), rtr.
+            iFrame "#".
+            iSplitR. done.
+            iSplitR. { iPureIntro; constructor; list_elem_of. }
+            (* TODO(Juliette): factor out this proof *)
+            iSplitL.
+              { iApply (big_sepL2_app with "[Hltr]").
+                - iApply (big_sepL2_singleton).
+                  iNext. rewrite triple_unfold.
+                  iExists b2, NONEV, bempty,
+                    o2, [], [],
+                    2, 0, [].
+                  iSplitR. { iPureIntro; eapply left_leaning; list_elem_of.  }
+                  do 2 doneL.
+                  iSplitR. isEmptyDeque.
+                  iSplitR. iApply bempty_spec.
+                  doneL.
+                  iPureIntro; simpl; aac_reflexivity.
+                - iApply (big_sepL2_mono with "Hltr").
+                  by auto.
+              }
+            iSplitR. iApply (big_sepL2_mono with "Hrtr"). by auto.
+            iPureIntro.
+            rewrite Heq Heq12 /=.
+            aac_reflexivity.
+          }
+          wp_pures.
+          iApply "Hψ".
+          iFrame.
+          ℓisDeque ℓ'. iExact "Hℓ'".
+        * apply bool_decide_eq_false_1 in Heqb0 as prNotFull.
+          wp_pures.
+          wp_bind (#ℓ <- _)%E.
+          wp_apply csref_store.
+          {
+            iSplit. iExact "Hℓ".
+            iFrame. by iApply (laterInFiveTuple with "Hv").
+          }
+          iIntros (unit).
+          wp_pures; clear unit.
+          wp_apply (bpush_spec with "Hpr") as "%pr' #Hpr'".
+          rewrite /assemble_.
+          wp_pures.
+          wp_bind (ref _)%E.
+          wp_apply (csref_alloc (fiveTuple (⋅x ++ oD))) as "%ℓ' #Hℓ'".
+          -- iExists pr', ld, md, rd, sf,
+              (⋅x ++ prC), ldC, mdC, rdC ,sfC,
+              (S kPr), kMd, kSf, ltr, rtr.
+            inversion cfg; [ exfalso; lia |].
+            assert (S kPr = kPr + 1) as -> by lia.
+            iFrame "#".
+            iSplitR. done.
+            iSplitR. { iPureIntro; constructor; invert_all_in; list_elem_of. }
+            iSplitR. iApply (big_sepL2_mono with "Hltr"). by auto.
+            iSplitR. iApply (big_sepL2_mono with "Hrtr"). by auto.
+            iPureIntro; rewrite Heq; aac_reflexivity.
+          -- wp_pures.
+            iApply "Hψ".
+            iFrame.
+            ℓisDeque ℓ'.
+            iExact "Hℓ'".
+  Qed.
+
+  Theorem push_spec oD (x : val) (d : val) :
+    {{{ IsDeque oD d }}}
+      push x d
+    {{{ d', RET d'; IsDeque (⋅x ++ oD) d' }}}.
+  Proof.
+    iIntros (ψ) "HD Hψ".
+    rewrite /IsDeque.
+    wp_apply (push_spec_helper with "[HD]") as "%d' HD'".
+      { iFrame. }
+    by iApply "Hψ".
+  Qed.
+
+End proof.
